@prefix ns1: <http://qudt.org/schema/qudt/> .
@prefix ns2: <http://data.ashrae.org/standard223#> .
@prefix owl: <http://www.w3.org/2002/07/owl#> .
@prefix rdf: <http://www.w3.org/1999/02/22-rdf-syntax-ns#> .
@prefix rdfs: <http://www.w3.org/2000/01/rdf-schema#> .
@prefix sh: <http://www.w3.org/ns/shacl#> .
@prefix skos: <http://www.w3.org/2004/02/skos/core#> .
@prefix xsd: <http://www.w3.org/2001/XMLSchema#> .

<urn:nawi-water-ontology#Class> a rdfs:Class,
        sh:NodeShape ;
    rdfs:label "Class"^^xsd:string ;
    rdfs:comment "This is a modeling construct. All classes defined in the watr ontology are instances of `watr:Class`."^^xsd:string ;
    rdfs:subClassOf rdfs:Class ;
    sh:property [ rdfs:comment "A `Class` must be associated with at least one label using the relation `rdfs:label`."^^xsd:string ;
            sh:minCount 1 ;
            sh:path rdfs:label ;
            sh:severity sh:Warning ] .

<urn:nawi-water-ontology#UnitProcess> a rdfs:Class ;
    rdfs:label "Unit Process"^^xsd:string ;
    rdfs:comment "A unit process is a specific type of water treatment process that can be applied to water."^^xsd:string ;
    rdfs:subClassOf ns2:Equipment,
        <urn:nawi-water-ontology#Class> ;
    sh:property [ sh:class <urn:nawi-water-ontology#Process> ;
            sh:message "A `Unit Process` must be associated with at least one water treatment process using the relation `watr:hasProcess`."^^xsd:string ;
            sh:minCount 1 ;
            sh:path <urn:nawi-water-ontology#hasProcess> ] .

<urn:nawi-water-ontology> a owl:Ontology ;
    owl:imports <http://data.ashrae.org/standard223/1.0/model/all>,
        <http://qudt.org/3.1.1/vocab/quantitykind>,
        <http://qudt.org/3.1.1/vocab/unit>,
        sh: .

<urn:nawi-water-ontology#AerationBasin> a sh:NodeShape,
        <urn:nawi-water-ontology#Class> ;
    rdfs:label "AerationBasin"^^xsd:string ;
    rdfs:comment "A tank where water is aerated to remove gases and volatile organic compounds"^^xsd:string ;
    rdfs:subClassOf <urn:nawi-water-ontology#Basin>,
        <urn:nawi-water-ontology#Reactor>,
        <urn:nawi-water-ontology#UnitProcess> ;
    sh:property [ sh:hasValue <urn:nawi-water-ontology#Process-GasTransfer> ;
            sh:maxCount 1 ;
            sh:message "Instances of AerationBasin must have the GasTransfer process."^^xsd:string ;
            sh:minCount 1 ;
            sh:path <urn:nawi-water-ontology#hasProcess> ] .

<urn:nawi-water-ontology#AerobicDigester> a sh:NodeShape,
        <urn:nawi-water-ontology#Class> ;
    rdfs:label "AerobicDigester"^^xsd:string ;
    rdfs:comment "A container to promote decomposition of organic waste in aerobic conditions"^^xsd:string ;
    rdfs:subClassOf <urn:nawi-water-ontology#Digester>,
        <urn:nawi-water-ontology#UnitProcess> ;
    sh:property [ sh:hasValue <urn:nawi-water-ontology#Process-AerobicDigestion> ;
            sh:maxCount 1 ;
            sh:message "Instances of AerobicDigester must have the AerobicDigestion process."^^xsd:string ;
            sh:minCount 1 ;
            sh:path <urn:nawi-water-ontology#hasProcess> ] .

<urn:nawi-water-ontology#AnaerobicDigester> a sh:NodeShape,
        <urn:nawi-water-ontology#Class> ;
    rdfs:label "AnaerobicDigester"^^xsd:string ;
    rdfs:comment "A container to promote decomposition of organic waste in anaerobic conditions"^^xsd:string ;
    rdfs:subClassOf <urn:nawi-water-ontology#Digester>,
        <urn:nawi-water-ontology#UnitProcess> ;
    sh:property [ sh:hasValue <urn:nawi-water-ontology#Process-AnaerobicDigestion> ;
            sh:maxCount 1 ;
            sh:message "Instances of AnaerobicDigester must have the AnaerobicDigestion process."^^xsd:string ;
            sh:minCount 1 ;
            sh:path <urn:nawi-water-ontology#hasProcess> ] .

<urn:nawi-water-ontology#Anode> a sh:NodeShape,
        <urn:nawi-water-ontology#Class> ;
    rdfs:label "Anode"^^xsd:string ;
    rdfs:comment "An electrode where oxidation occurs, often a sacrificial component in electrocoagulation."^^xsd:string ;
    rdfs:subClassOf <urn:nawi-water-ontology#Electrode> .

<urn:nawi-water-ontology#Battery> a sh:NodeShape,
        <urn:nawi-water-ontology#Class> ;
    rdfs:label "Battery"^^xsd:string ;
    rdfs:comment "A device that stores energy for later use"^^xsd:string ;
    rdfs:subClassOf ns2:Battery .

<urn:nawi-water-ontology#BiologicalAeratedFilter> a sh:NodeShape,
        <urn:nawi-water-ontology#Class> ;
    rdfs:label "Biological Aerated Filter (BAF)"^^xsd:string ;
    rdfs:comment "A filter that uses biological processes to remove contaminants."^^xsd:string ;
    rdfs:subClassOf <urn:nawi-water-ontology#Filter>,
        <urn:nawi-water-ontology#UnitProcess> ;
    sh:property [ sh:hasValue <urn:nawi-water-ontology#Process-BiologicallyActiveFiltration> ;
            sh:maxCount 1 ;
            sh:message "Instances of BiologicalAeratedFilter must have the BiologicallyActiveFiltration process."^^xsd:string ;
            sh:minCount 1 ;
            sh:path <urn:nawi-water-ontology#hasProcess> ] .

<urn:nawi-water-ontology#Boiler> a sh:NodeShape,
        <urn:nawi-water-ontology#Class> ;
    rdfs:label "Boiler"^^xsd:string ;
    rdfs:comment "A device for heating water"^^xsd:string ;
    rdfs:subClassOf ns2:Boiler .

<urn:nawi-water-ontology#CartridgeFiltrationUnit> a sh:NodeShape,
        <urn:nawi-water-ontology#Class> ;
    rdfs:label "CartridgeFiltrationUnit"^^xsd:string ;
    rdfs:comment "A filter system using a cartridge to remove contaminants from fluids"^^xsd:string ;
    rdfs:subClassOf <urn:nawi-water-ontology#Filter> .

<urn:nawi-water-ontology#Cathode> a sh:NodeShape,
        <urn:nawi-water-ontology#Class> ;
    rdfs:label "Cathode"^^xsd:string ;
    rdfs:comment "An electrode where reduction occurs."^^xsd:string ;
    rdfs:subClassOf <urn:nawi-water-ontology#Electrode> .

<urn:nawi-water-ontology#CentrifugalThickener> a sh:NodeShape,
        <urn:nawi-water-ontology#Class> ;
    rdfs:label "CentrifugalThickener"^^xsd:string ;
    rdfs:comment "A thickener that uses centrifugal force to separate solids from liquids"^^xsd:string ;
    rdfs:subClassOf <urn:nawi-water-ontology#Thickener>,
        <urn:nawi-water-ontology#UnitProcess> ;
    sh:property [ sh:hasValue <urn:nawi-water-ontology#Process-Centrifugation> ;
            sh:maxCount 1 ;
            sh:message "Instances of CentrifugalThickener must have the Centrifugation process."^^xsd:string ;
            sh:minCount 1 ;
            sh:path <urn:nawi-water-ontology#hasProcess> ] .

<urn:nawi-water-ontology#CheckValve> a ns2:Class,
        sh:NodeShape,
        <urn:nawi-water-ontology#Class> ;
    rdfs:label "Check Valve"^^xsd:string ;
    rdfs:subClassOf ns2:Valve .

<urn:nawi-water-ontology#ChlorinationBasin> a sh:NodeShape,
        <urn:nawi-water-ontology#Class> ;
    rdfs:label "ChlorinationBasin"^^xsd:string ;
    rdfs:comment "A basin where chlorine is added for disinfection"^^xsd:string ;
    rdfs:subClassOf <urn:nawi-water-ontology#Basin>,
        <urn:nawi-water-ontology#ChlorinationUnit> .

<urn:nawi-water-ontology#CoagulationBasin> a sh:NodeShape,
        <urn:nawi-water-ontology#Class> ;
    rdfs:label "CoagulationBasin"^^xsd:string ;
    rdfs:comment "A basin where coagulation occurs to destabilize particles in water"^^xsd:string ;
    rdfs:subClassOf <urn:nawi-water-ontology#Basin>,
        <urn:nawi-water-ontology#UnitProcess> ;
    sh:property [ sh:hasValue <urn:nawi-water-ontology#Process-Coagulation> ;
            sh:maxCount 1 ;
            sh:message "Instances of CoagulationBasin must have the Coagulation process."^^xsd:string ;
            sh:minCount 1 ;
            sh:path <urn:nawi-water-ontology#hasProcess> ] .

<urn:nawi-water-ontology#Cogenerator> a sh:NodeShape,
        <urn:nawi-water-ontology#Class> ;
    rdfs:label "Cogenerator"^^xsd:string ;
    rdfs:comment "An equipment that produces both electricity and heat from the same energy source"^^xsd:string ;
    rdfs:subClassOf ns2:Equipment .

<urn:nawi-water-ontology#Compressor> a sh:NodeShape,
        <urn:nawi-water-ontology#Class> ;
    rdfs:label "Compressor"^^xsd:string ;
    rdfs:comment "An equipment that increases the pressure of a gas"^^xsd:string ;
    rdfs:subClassOf ns2:Compressor .

<urn:nawi-water-ontology#Condenser> a sh:NodeShape,
        <urn:nawi-water-ontology#Class> ;
    rdfs:label "Condenser"^^xsd:string ;
    rdfs:comment "A device used to condense a gaseous substance back into a liquid"^^xsd:string ;
    rdfs:subClassOf ns2:HeatExchanger,
        <urn:nawi-water-ontology#UnitProcess> ;
    sh:property [ sh:hasValue <urn:nawi-water-ontology#Process-Condensation> ;
            sh:maxCount 1 ;
            sh:message "Instances of Condenser must have the Condensation process."^^xsd:string ;
            sh:minCount 1 ;
            sh:path <urn:nawi-water-ontology#hasProcess> ] .

<urn:nawi-water-ontology#Conditioner> a sh:NodeShape,
        <urn:nawi-water-ontology#Class> ;
    rdfs:label "Conditioner"^^xsd:string ;
    rdfs:comment "An equipment used to prepare raw biogas from a digester by removing impurities"^^xsd:string ;
    rdfs:subClassOf ns2:Equipment .

<urn:nawi-water-ontology#ConductivitySensor> a sh:NodeShape,
        <urn:nawi-water-ontology#Class> ;
    rdfs:label "ConductivitySensor"^^xsd:string ;
    rdfs:comment "A sensor used to measure the electrical conductivity of a solution"^^xsd:string ;
    rdfs:subClassOf <urn:nawi-water-ontology#Sensor> .

<urn:nawi-water-ontology#ContinuouslyStirredTankReactor> a sh:NodeShape,
        <urn:nawi-water-ontology#Class> ;
    rdfs:label "ContinuouslyStirredTankReactor"^^xsd:string ;
    rdfs:comment "A reactor in which contents are well mixed and reactants are added continuously"^^xsd:string ;
    rdfs:subClassOf <urn:nawi-water-ontology#Reactor> .

<urn:nawi-water-ontology#Controller> a ns2:Class,
        sh:NodeShape,
        <urn:nawi-water-ontology#Class> ;
    rdfs:label "Controller"^^xsd:string ;
    rdfs:subClassOf ns2:Controller .

<urn:nawi-water-ontology#Crystallizer> a sh:NodeShape,
        <urn:nawi-water-ontology#Class> ;
    rdfs:label "Crystallizer"^^xsd:string ;
    rdfs:comment "An equipment used to produce solid crystals from a solution"^^xsd:string ;
    rdfs:subClassOf ns2:Equipment,
        <urn:nawi-water-ontology#UnitProcess> ;
    sh:property [ sh:hasValue <urn:nawi-water-ontology#Process-Crystallization> ;
            sh:maxCount 1 ;
            sh:message "Instances of Crystallizer must have the Crystallization process."^^xsd:string ;
            sh:minCount 1 ;
            sh:path <urn:nawi-water-ontology#hasProcess> ] .

<urn:nawi-water-ontology#DMERecoverySystem> a sh:NodeShape,
        <urn:nawi-water-ontology#Class> ;
    rdfs:label "Dimethyl Ether (DME) Recovery System"^^xsd:string ;
    rdfs:comment "A system designed to recover a high percentage of Dimethyl Ether solvent in solvent-driven processes."^^xsd:string ;
    rdfs:subClassOf ns2:Equipment .

<urn:nawi-water-ontology#DewateringUnit> a sh:NodeShape,
        <urn:nawi-water-ontology#Class> ;
    rdfs:label "Dewatering"^^xsd:string ;
    rdfs:comment "A unit used to remove water from solid material"^^xsd:string ;
    rdfs:subClassOf ns2:Equipment,
        <urn:nawi-water-ontology#UnitProcess> ;
    sh:property [ sh:hasValue <urn:nawi-water-ontology#Process-Dewatering> ;
            sh:maxCount 1 ;
            sh:message "Instances of DewateringUnit must have the Dewatering process."^^xsd:string ;
            sh:minCount 1 ;
            sh:path <urn:nawi-water-ontology#hasProcess> ] .

<urn:nawi-water-ontology#DissolvedAirFlotationThickener> a sh:NodeShape,
        <urn:nawi-water-ontology#Class> ;
    rdfs:label "DissolvedAirFlotationThickener"^^xsd:string ;
    rdfs:comment "A thickener that uses dissolved air to separate solids from liquids"^^xsd:string ;
    rdfs:subClassOf <urn:nawi-water-ontology#Thickener>,
        <urn:nawi-water-ontology#UnitProcess> ;
    sh:property [ sh:hasValue <urn:nawi-water-ontology#Process-Flotation> ;
            sh:maxCount 1 ;
            sh:message "Instances of DissolvedAirFlotationThickener must have the Flotation process."^^xsd:string ;
            sh:minCount 1 ;
            sh:path <urn:nawi-water-ontology#hasProcess> ] .

<urn:nawi-water-ontology#EfficiencySensor> a sh:NodeShape,
        <urn:nawi-water-ontology#Class> ;
    rdfs:label "EfficiencySensor"^^xsd:string ;
    rdfs:comment "A sensor used to measure the efficiency of a system or equipment"^^xsd:string ;
    rdfs:subClassOf ns2:Sensor .

<urn:nawi-water-ontology#ElectricallyConductingMembrane> a sh:NodeShape,
        <urn:nawi-water-ontology#Class> ;
    rdfs:label "Electrically Conducting Membrane"^^xsd:string ;
    rdfs:comment "A membrane capable of conducting electricity, used for in-situ cleaning or electro-oxidation processes."^^xsd:string ;
    rdfs:subClassOf <urn:nawi-water-ontology#Filter> .

<urn:nawi-water-ontology#ElectroDialyticCrystallizer> a sh:NodeShape,
        <urn:nawi-water-ontology#Class> ;
    rdfs:label "Electro-Dialytic Crystallizer (EDC)"^^xsd:string ;
    rdfs:comment "A modular system designed for brine concentration and crystallization, integrating electrodialysis and crystallization."^^xsd:string ;
    rdfs:subClassOf ns2:Equipment,
        <urn:nawi-water-ontology#UnitProcess> ;
    sh:property [ sh:hasValue <urn:nawi-water-ontology#Process-Electrodialysis> ;
            sh:maxCount 1 ;
            sh:message "Instances of ElectroDialyticCrystallizer must have the Electrodialysis process."^^xsd:string ;
            sh:minCount 1 ;
            sh:path <urn:nawi-water-ontology#hasProcess> ],
        [ sh:hasValue <urn:nawi-water-ontology#Process-Crystallization> ;
            sh:maxCount 1 ;
            sh:message "Instances of ElectroDialyticCrystallizer must have the Crystallization process."^^xsd:string ;
            sh:minCount 1 ;
            sh:path <urn:nawi-water-ontology#hasProcess> ] .

<urn:nawi-water-ontology#ElectrocoagulationUnit> a sh:NodeShape,
        <urn:nawi-water-ontology#Class> ;
    rdfs:label "Electrocoagulation Unit"^^xsd:string ;
    rdfs:comment "A unit that uses electrocoagulation for contaminant removal."^^xsd:string ;
    rdfs:subClassOf ns2:Equipment,
        <urn:nawi-water-ontology#UnitProcess> ;
    sh:property [ sh:hasValue <urn:nawi-water-ontology#Process-Electrocoagulation> ;
            sh:maxCount 1 ;
            sh:message "Instances of ElectrocoagulationUnit must have the Electrocoagulation process."^^xsd:string ;
            sh:minCount 1 ;
            sh:path <urn:nawi-water-ontology#hasProcess> ] .

<urn:nawi-water-ontology#ElectrodialysisUnit> a sh:NodeShape,
        <urn:nawi-water-ontology#Class> ;
    rdfs:label "Electrodialysis"^^xsd:string ;
    rdfs:comment "A unit that uses electricity to drive ion movement through a membrane"^^xsd:string ;
    rdfs:subClassOf ns2:Equipment,
        <urn:nawi-water-ontology#UnitProcess> ;
    sh:property [ sh:hasValue <urn:nawi-water-ontology#Process-Electrodialysis> ;
            sh:maxCount 1 ;
            sh:message "Instances of ElectrodialysisUnit must have the Electrodialysis process."^^xsd:string ;
            sh:minCount 1 ;
            sh:path <urn:nawi-water-ontology#hasProcess> ] .

<urn:nawi-water-ontology#Electrolyzer> a sh:NodeShape,
        <urn:nawi-water-ontology#Class> ;
    rdfs:label "Electrolyzer"^^xsd:string ;
    rdfs:comment "An equipment that uses electricity to split liquids into constituent elements"^^xsd:string ;
    rdfs:subClassOf ns2:Equipment,
        <urn:nawi-water-ontology#UnitProcess> ;
    sh:property [ sh:hasValue <urn:nawi-water-ontology#Process-Electrolysis> ;
            sh:maxCount 1 ;
            sh:message "Instances of Electrolyzer must have the Electrolysis process."^^xsd:string ;
            sh:minCount 1 ;
            sh:path <urn:nawi-water-ontology#hasProcess> ] .

<urn:nawi-water-ontology#ElectromagneticFieldDevice> a sh:NodeShape,
        <urn:nawi-water-ontology#Class> ;
    rdfs:label "Electromagnetic Field (EMF) Device"^^xsd:string ;
    rdfs:comment "A device that generates an electromagnetic field, used as a pretreatment method for membrane scaling and fouling control."^^xsd:string ;
    rdfs:subClassOf ns2:Equipment .

<urn:nawi-water-ontology#Evaporator> a sh:NodeShape,
        <urn:nawi-water-ontology#Class> ;
    rdfs:label "Evaporator"^^xsd:string ;
    rdfs:comment "A device used to turn the liquid form of a substance into its gaseous form"^^xsd:string ;
    rdfs:subClassOf ns2:HeatExchanger,
        <urn:nawi-water-ontology#UnitProcess> ;
    sh:property [ sh:hasValue <urn:nawi-water-ontology#Process-Evaporation> ;
            sh:maxCount 1 ;
            sh:message "Instances of Evaporator must have the Evaporation process."^^xsd:string ;
            sh:minCount 1 ;
            sh:path <urn:nawi-water-ontology#hasProcess> ] .

<urn:nawi-water-ontology#Flare> a sh:NodeShape,
        <urn:nawi-water-ontology#Class> ;
    rdfs:label "Flare"^^xsd:string ;
    rdfs:comment "A device used to burn off unwanted gas"^^xsd:string ;
    rdfs:subClassOf ns2:Equipment .

<urn:nawi-water-ontology#FlocculationBasin> a sh:NodeShape,
        <urn:nawi-water-ontology#Class> ;
    rdfs:label "FlocculationBasin"^^xsd:string ;
    rdfs:comment "A tank where flocculation occurs to aggregate particles in water"^^xsd:string ;
    rdfs:subClassOf <urn:nawi-water-ontology#Basin>,
        <urn:nawi-water-ontology#UnitProcess> ;
    sh:property [ sh:hasValue <urn:nawi-water-ontology#Process-Flocculation> ;
            sh:maxCount 1 ;
            sh:message "Instances of FlocculationBasin must have the Flocculation process."^^xsd:string ;
            sh:minCount 1 ;
            sh:path <urn:nawi-water-ontology#hasProcess> ] .

<urn:nawi-water-ontology#FlowSensor> a sh:NodeShape,
        <urn:nawi-water-ontology#Class> ;
    rdfs:label "FlowSensor"^^xsd:string ;
    rdfs:comment "A sensor used to measure the flow rate of liquids or gases"^^xsd:string ;
    rdfs:subClassOf ns2:FlowSensor .

<urn:nawi-water-ontology#FrequencySensor> a sh:NodeShape,
        <urn:nawi-water-ontology#Class> ;
    rdfs:label "Frequency Sensor"^^xsd:string ;
    rdfs:comment "A sensor used to measure the frequency of a signal or mechanical vibration"^^xsd:string ;
    rdfs:subClassOf ns2:Sensor .

<urn:nawi-water-ontology#GranulatedActivatedCarbonAdsorber> a sh:NodeShape,
        <urn:nawi-water-ontology#Class> ;
    rdfs:label "Granulated Activated Carbon (GAC) Adsorber"^^xsd:string ;
    rdfs:comment "A unit that uses granulated activated carbon to adsorb impurities from water."^^xsd:string ;
    rdfs:subClassOf ns2:Equipment,
        <urn:nawi-water-ontology#UnitProcess> ;
    sh:property [ sh:hasValue <urn:nawi-water-ontology#Process-GranulatedActivatedCarbonAdsorption> ;
            sh:maxCount 1 ;
            sh:message "Instances of GranulatedActivatedCarbonAdsorber must have the GranulatedActivatedCarbonAdsorption process."^^xsd:string ;
            sh:minCount 1 ;
            sh:path <urn:nawi-water-ontology#hasProcess> ] .

<urn:nawi-water-ontology#GravityBeltThickener> a sh:NodeShape,
        <urn:nawi-water-ontology#Class> ;
    rdfs:label "Gravity Belt Thickener"^^xsd:string ;
    rdfs:comment "A thickener that combines gravity separation with a belt system"^^xsd:string ;
    rdfs:subClassOf <urn:nawi-water-ontology#BeltThickener> .

<urn:nawi-water-ontology#GravityThickener> a sh:NodeShape,
        <urn:nawi-water-ontology#Class> ;
    rdfs:label "GravityThickener"^^xsd:string ;
    rdfs:comment "A thickener that uses gravity to separate solids from liquids"^^xsd:string ;
    rdfs:subClassOf <urn:nawi-water-ontology#Thickener>,
        <urn:nawi-water-ontology#UnitProcess> ;
    sh:property [ sh:hasValue <urn:nawi-water-ontology#Process-Sedimentation> ;
            sh:maxCount 1 ;
            sh:message "Instances of GravityThickener must have the Sedimentation process."^^xsd:string ;
            sh:minCount 1 ;
            sh:path <urn:nawi-water-ontology#hasProcess> ] .

<urn:nawi-water-ontology#GritChamber> a sh:NodeShape,
        <urn:nawi-water-ontology#Class> ;
    rdfs:label "Grit Chamber"^^xsd:string ;
    rdfs:comment "A chamber used to remove grit from wastewater"^^xsd:string ;
    rdfs:subClassOf ns2:Equipment,
        <urn:nawi-water-ontology#UnitProcess> ;
    sh:property [ sh:hasValue <urn:nawi-water-ontology#Process-Sedimentation> ;
            sh:maxCount 1 ;
            sh:message "Instances of GritChamber must have the Sedimentation process."^^xsd:string ;
            sh:minCount 1 ;
            sh:path <urn:nawi-water-ontology#hasProcess> ] .

<urn:nawi-water-ontology#IonExchangeMembrane> a sh:NodeShape,
        <urn:nawi-water-ontology#Class> ;
    rdfs:label "IonExchangeMembrane"^^xsd:string ;
    rdfs:comment "A membrane that selectively allows ions to pass through while blocking other substances"^^xsd:string ;
    rdfs:subClassOf ns2:Equipment,
        <urn:nawi-water-ontology#UnitProcess> ;
    sh:property [ sh:hasValue <urn:nawi-water-ontology#Process-IonExchange> ;
            sh:maxCount 1 ;
            sh:message "Instances of IonExchangeMembrane must have the IonExchange process."^^xsd:string ;
            sh:minCount 1 ;
            sh:path <urn:nawi-water-ontology#hasProcess> ] .

<urn:nawi-water-ontology#LevelSensor> a sh:NodeShape,
        <urn:nawi-water-ontology#Class> ;
    rdfs:label "LevelSensor"^^xsd:string ;
    rdfs:comment "A sensor used to detect the level of liquids or solids in a tank"^^xsd:string ;
    rdfs:subClassOf ns2:Sensor .

<urn:nawi-water-ontology#ManualMeasurementPort> a sh:NodeShape,
        <urn:nawi-water-ontology#Class> ;
    rdfs:label "Manual Measurement Port"^^xsd:string ;
    rdfs:comment "A location where manual measurements are taken"^^xsd:string ;
    rdfs:subClassOf ns2:Sensor .

<urn:nawi-water-ontology#MembraneBioreactor> a sh:NodeShape,
        <urn:nawi-water-ontology#Class> ;
    rdfs:label "MembraneBioreactor"^^xsd:string ;
    rdfs:comment "A filter system that combines a membrane process like microfiltration with a biological reactor"^^xsd:string ;
    rdfs:subClassOf <urn:nawi-water-ontology#Filter>,
        <urn:nawi-water-ontology#UnitProcess> ;
    sh:property [ sh:hasValue <urn:nawi-water-ontology#Process-MembraneBioreactor> ;
            sh:maxCount 1 ;
            sh:message "Instances of MembraneBioreactor must have the MembraneBioreactor process."^^xsd:string ;
            sh:minCount 1 ;
            sh:path <urn:nawi-water-ontology#hasProcess> ] .

<urn:nawi-water-ontology#MicrofiltrationUnit> a sh:NodeShape,
        <urn:nawi-water-ontology#Class> ;
    rdfs:label "MicrofiltrationUnit"^^xsd:string ;
    rdfs:comment "A filter system which removes contaminants from a liquid by passing it through a microporous membrane"^^xsd:string ;
    rdfs:subClassOf <urn:nawi-water-ontology#Filter> .

<urn:nawi-water-ontology#MolybdenumSulfideBasedMembrane> a sh:NodeShape,
        <urn:nawi-water-ontology#Class> ;
    rdfs:label "Molybdenum Sulfide (MoS2)-based Membrane"^^xsd:string ;
    rdfs:comment "A specific material demonstrating effectiveness in removing heavy metals and oxyanions with high selectivity."^^xsd:string ;
    rdfs:subClassOf <urn:nawi-water-ontology#Filter> .

<urn:nawi-water-ontology#MultifunctionalMembrane> a sh:NodeShape,
        <urn:nawi-water-ontology#Class> ;
    rdfs:label "Multifunctional Membrane"^^xsd:string ;
    rdfs:comment "A membrane integrating multiple processes (e.g., reduction, adsorption, filtration) for selective removal and recovery of contaminants."^^xsd:string ;
    rdfs:subClassOf <urn:nawi-water-ontology#Filter> .

<urn:nawi-water-ontology#NanofiltrationUnit> a sh:NodeShape,
        <urn:nawi-water-ontology#Class> ;
    rdfs:label "NanofiltrationUnit"^^xsd:string ;
    rdfs:comment "A filter system that uses a membrane to soften water and remove organic contaminants"^^xsd:string ;
    rdfs:subClassOf <urn:nawi-water-ontology#Filter> .

<urn:nawi-water-ontology#OxygenDemandSensor> a sh:NodeShape,
        <urn:nawi-water-ontology#Class> ;
    rdfs:label "OxygenDemandSensor"^^xsd:string ;
    rdfs:comment "A sensor used to measure Chemical Oxygen Demand (COD) and Biological Oxygen Demand (BOD)"^^xsd:string ;
    rdfs:subClassOf ns2:Sensor .

<urn:nawi-water-ontology#OxygenMeter> a sh:NodeShape,
        <urn:nawi-water-ontology#Class> ;
    rdfs:label "Oxygen Meter"^^xsd:string ;
    rdfs:comment "A sensor used to measure the concentration of oxygen"^^xsd:string ;
    rdfs:subClassOf ns2:ConcentrationSensor .

<urn:nawi-water-ontology#OzonationUnit> a sh:NodeShape,
        <urn:nawi-water-ontology#Class> ;
    rdfs:label "Ozonation Unit"^^xsd:string ;
    rdfs:comment "A unit that uses ozone for water treatment."^^xsd:string ;
    rdfs:subClassOf ns2:Equipment,
        <urn:nawi-water-ontology#UnitProcess> ;
    sh:property [ sh:hasValue <urn:nawi-water-ontology#Process-Ozonation> ;
            sh:maxCount 1 ;
            sh:message "Instances of OzonationUnit must have the Ozonation process."^^xsd:string ;
            sh:minCount 1 ;
            sh:path <urn:nawi-water-ontology#hasProcess> ] .

<urn:nawi-water-ontology#PlugFlowReactor> a sh:NodeShape,
        <urn:nawi-water-ontology#Class> ;
    rdfs:label "PlugFlowReactor"^^xsd:string ;
    rdfs:comment "A type of reactor where the fluid flows in one direction through the tube"^^xsd:string ;
    rdfs:subClassOf <urn:nawi-water-ontology#Reactor> ;
    sh:property [ rdfs:comment "A plug flow reactor has at least one inlet fluid connection point"^^xsd:string ;
            sh:path ns2:hasConnectionPoint ;
            sh:qualifiedMinCount 1 ;
            sh:qualifiedValueShape [ sh:class ns2:InletConnectionPoint ;
                    sh:property [ sh:hasValue ns2:Mix-Fluid ;
                            sh:path ns2:hasMedium ] ] ],
        [ rdfs:comment "A plug flow reactor has at least one outlet fluid connection point"^^xsd:string ;
            sh:path ns2:hasConnectionPoint ;
            sh:qualifiedMinCount 1 ;
            sh:qualifiedValueShape [ sh:class ns2:OutletConnectionPoint ;
                    sh:property [ sh:hasValue ns2:Mix-Fluid ;
                            sh:path ns2:hasMedium ] ] ] .

<urn:nawi-water-ontology#Pond> a sh:NodeShape,
        <urn:nawi-water-ontology#Class> ;
    rdfs:label "Pond"^^xsd:string ;
    rdfs:comment "A body of still water smaller than a lake, used for treatment or storage"^^xsd:string ;
    rdfs:subClassOf ns2:Equipment .

<urn:nawi-water-ontology#PressureExchanger> a sh:NodeShape,
        <urn:nawi-water-ontology#Class> ;
    rdfs:label "PressureExchanger"^^xsd:string ;
    rdfs:comment "A device used to transfer pressure energy from one fluid to another"^^xsd:string ;
    rdfs:subClassOf ns2:Equipment .

<urn:nawi-water-ontology#PressureSensor> a sh:NodeShape,
        <urn:nawi-water-ontology#Class> ;
    rdfs:label "PressureSensor"^^xsd:string ;
    rdfs:comment "A sensor used to measure pressure"^^xsd:string ;
    rdfs:subClassOf ns2:PressureSensor .

<urn:nawi-water-ontology#ProcessType> a sh:NodeShape,
        <urn:nawi-water-ontology#Class> ;
    rdfs:label "Water Process"^^xsd:string ;
    skos:definition "A process applied to water treatment."^^xsd:string ;
    sh:property [ sh:datatype xsd:string ;
            sh:description "A human-readable definition of the process type."^^xsd:string ;
            sh:maxCount 1 ;
            sh:minCount 1 ;
            sh:path skos:definition ],
        [ sh:datatype xsd:string ;
            sh:description "A human-readable label for the process type."^^xsd:string ;
            sh:maxCount 1 ;
            sh:minCount 1 ;
            sh:path rdfs:label ] .

<urn:nawi-water-ontology#Pump> a sh:NodeShape,
        <urn:nawi-water-ontology#Class> ;
    rdfs:label "Pump"^^xsd:string ;
    rdfs:comment "A device used to move fluids by mechanical action"^^xsd:string ;
    rdfs:subClassOf ns2:Pump .

<urn:nawi-water-ontology#RapidSandFilter> a sh:NodeShape,
        <urn:nawi-water-ontology#Class> ;
    rdfs:label "Rapid Sand Filter"^^xsd:string ;
    rdfs:comment "A type of media filter that uses sand as the filter medium and operates at high filtration rates."^^xsd:string ;
    rdfs:subClassOf <urn:nawi-water-ontology#MediaFiltration> ;
    sh:property [ sh:hasValue <urn:nawi-water-ontology#Process-RapidSandFiltration> ;
            sh:maxCount 1 ;
            sh:message "Instances of RapidSandFilter must have the RapidSandFiltration process."^^xsd:string ;
            sh:minCount 1 ;
            sh:path <urn:nawi-water-ontology#hasProcess> ] .

<urn:nawi-water-ontology#Reservoir> a sh:NodeShape,
        <urn:nawi-water-ontology#Class> ;
    rdfs:label "Reservoir"^^xsd:string ;
    rdfs:comment "A large natural or artificial body of water used for water supply"^^xsd:string ;
    rdfs:subClassOf ns2:Equipment .

<urn:nawi-water-ontology#ReverseOsmosisMembrane> a sh:NodeShape,
        <urn:nawi-water-ontology#Class> ;
    rdfs:label "ReverseOsmosisMembrane"^^xsd:string ;
    rdfs:comment "A membrane used for reverse osmosis"^^xsd:string ;
    rdfs:subClassOf <urn:nawi-water-ontology#Filter> .

<urn:nawi-water-ontology#RotaryDrumThickener> a sh:NodeShape,
        <urn:nawi-water-ontology#Class> ;
    rdfs:label "Rotary Drum Thickener"^^xsd:string ;
    rdfs:comment "A thickener that uses a rotating drum to separate solids from liquids"^^xsd:string ;
    rdfs:subClassOf <urn:nawi-water-ontology#Thickener>,
        <urn:nawi-water-ontology#UnitProcess> ;
    sh:property [ sh:hasValue <urn:nawi-water-ontology#Process-Filtration> ;
            sh:maxCount 1 ;
            sh:message "Instances of RotaryDrumThickener must have the Filtration process."^^xsd:string ;
            sh:minCount 1 ;
            sh:path <urn:nawi-water-ontology#hasProcess> ] .

<urn:nawi-water-ontology#RotationSensor> a sh:NodeShape,
        <urn:nawi-water-ontology#Class> ;
    rdfs:label "RotationSensor"^^xsd:string ;
    rdfs:comment "A sensor used to measure the rotational speed or position of an object"^^xsd:string ;
    rdfs:subClassOf ns2:Sensor .

<urn:nawi-water-ontology#Screen> a sh:NodeShape,
        <urn:nawi-water-ontology#Class> ;
    rdfs:label "Screen"^^xsd:string ;
    rdfs:comment "An equipment used for separation"^^xsd:string ;
    rdfs:subClassOf ns2:Equipment,
        <urn:nawi-water-ontology#UnitProcess> ;
    sh:property [ sh:hasValue <urn:nawi-water-ontology#Process-Screening> ;
            sh:maxCount 1 ;
            sh:message "Instances of Screen must have the Screening process."^^xsd:string ;
            sh:minCount 1 ;
            sh:path <urn:nawi-water-ontology#hasProcess> ] .

<urn:nawi-water-ontology#SedimentationTank> a sh:NodeShape,
        <urn:nawi-water-ontology#Class> ;
    rdfs:label "SedimentationTank"^^xsd:string ;
    rdfs:comment "A tank used to remove solids from liquids through sedimentation"^^xsd:string ;
    rdfs:subClassOf <urn:nawi-water-ontology#Tank>,
        <urn:nawi-water-ontology#UnitProcess> ;
    sh:property [ sh:hasValue <urn:nawi-water-ontology#Process-Sedimentation> ;
            sh:maxCount 1 ;
            sh:message "Instances of SedimentationTank must have the Sedimentation process."^^xsd:string ;
            sh:minCount 1 ;
            sh:path <urn:nawi-water-ontology#hasProcess> ] .

<urn:nawi-water-ontology#SequencingBatchReactor> a sh:NodeShape,
        <urn:nawi-water-ontology#Class> ;
    rdfs:label "SequencingBatchReactor"^^xsd:string ;
    rdfs:comment "A type of activated sludge process for wastewater treatment"^^xsd:string ;
    rdfs:subClassOf <urn:nawi-water-ontology#Reactor>,
        <urn:nawi-water-ontology#UnitProcess> ;
    sh:property [ sh:hasValue <urn:nawi-water-ontology#Process-ActivatedSludge> ;
            sh:maxCount 1 ;
            sh:message "Instances of SequencingBatchReactor must have the ActivatedSludge process."^^xsd:string ;
            sh:minCount 1 ;
            sh:path <urn:nawi-water-ontology#hasProcess> ],
        [ rdfs:comment "A SBR has at least 1 sludge return point"^^xsd:string ;
            sh:path ns2:hasConnectionPoint ;
            sh:qualifiedMinCount 1 ;
            sh:qualifiedValueShape [ sh:class ns2:OutletConnectionPoint ;
                    sh:property [ sh:hasValue ns2:Fluid-Sludge ;
                            sh:path ns2:hasMedium ] ] ] ;
    sh:xone ( [ sh:property [ rdfs:comment "A SBR has at least 1 outlet fluid connection point"^^xsd:string ;
                        sh:path ns2:hasConnectionPoint ;
                        sh:qualifiedMinCount 1 ;
                        sh:qualifiedValueShape [ sh:class ns2:OutletConnectionPoint ;
                                sh:property [ sh:hasValue ns2:Mix-Fluid ;
                                        sh:path ns2:hasMedium ] ] ],
                    [ rdfs:comment "A SBR has at least 1 inlet fluid connection point"^^xsd:string ;
                        sh:path ns2:hasConnectionPoint ;
                        sh:qualifiedMinCount 1 ;
                        sh:qualifiedValueShape [ sh:class ns2:InletConnectionPoint ;
                                sh:property [ sh:hasValue ns2:Mix-Fluid ;
                                        sh:path ns2:hasMedium ] ] ] ] [ sh:property [ rdfs:comment "A SBR has at least 1 bidirectional fluid connection point"^^xsd:string ;
                        sh:path ns2:hasConnectionPoint ;
                        sh:qualifiedMinCount 1 ;
                        sh:qualifiedValueShape [ sh:class ns2:BidirectionalConnectionPoint ;
                                sh:property [ sh:hasValue ns2:Mix-Fluid ;
                                        sh:path ns2:hasMedium ] ] ] ] ) .

<urn:nawi-water-ontology#SolventExtractionSystem> a sh:NodeShape,
        <urn:nawi-water-ontology#Class> ;
    rdfs:label "Solvent Extraction System"^^xsd:string ;
    rdfs:comment "A system that uses a solvent to selectively extract water from highly saline brines."^^xsd:string ;
    rdfs:subClassOf ns2:Equipment,
        <urn:nawi-water-ontology#UnitProcess> ;
    sh:property [ sh:hasValue <urn:nawi-water-ontology#Process-SolventExtraction> ;
            sh:maxCount 1 ;
            sh:message "Instances of SolventExtractionSystem must have the SolventExtraction process."^^xsd:string ;
            sh:minCount 1 ;
            sh:path <urn:nawi-water-ontology#hasProcess> ] .

<urn:nawi-water-ontology#SpeedSensor> a sh:NodeShape,
        <urn:nawi-water-ontology#Class> ;
    rdfs:label "Speed Sensor"^^xsd:string ;
    rdfs:comment "A sensor used to measure the speed of an object or fluid"^^xsd:string ;
    rdfs:subClassOf ns2:Sensor .

<urn:nawi-water-ontology#StandardizedFlowCell> a sh:NodeShape,
        <urn:nawi-water-ontology#Class> ;
    rdfs:label "Standardized Flow Cell"^^xsd:string ;
    rdfs:comment "An experimental apparatus developed for research experiments, for example in Electrocoagulation (EC), in continuous flow mode."^^xsd:string ;
    rdfs:subClassOf ns2:Equipment .

<urn:nawi-water-ontology#StateOfChargeSensor> a sh:NodeShape,
        <urn:nawi-water-ontology#Class> ;
    rdfs:label "State of Charge Sensor"^^xsd:string ;
    rdfs:comment "A sensor used to measure the remaining charge in a battery or energy storage system"^^xsd:string ;
    rdfs:subClassOf ns2:Sensor .

<urn:nawi-water-ontology#StaticMixer> a sh:NodeShape,
        <urn:nawi-water-ontology#Class> ;
    rdfs:label "StaticMixer"^^xsd:string ;
    rdfs:comment "A device for mixing liquids without moving components"^^xsd:string ;
    rdfs:subClassOf <urn:nawi-water-ontology#Reactor>,
        <urn:nawi-water-ontology#UnitProcess> ;
    sh:property [ sh:hasValue <urn:nawi-water-ontology#Process-Mixing> ;
            sh:maxCount 1 ;
            sh:message "Instances of StaticMixer must have the Mixing process."^^xsd:string ;
            sh:minCount 1 ;
            sh:path <urn:nawi-water-ontology#hasProcess> ] .

<urn:nawi-water-ontology#TemperatureSensor> a sh:NodeShape,
        <urn:nawi-water-ontology#Class> ;
    rdfs:label "TemperatureSensor"^^xsd:string ;
    rdfs:comment "A sensor used to measure temperature"^^xsd:string ;
    rdfs:subClassOf ns2:TemperatureSensor .

<urn:nawi-water-ontology#ThreeWayValve> a ns2:Class,
        sh:NodeShape,
        <urn:nawi-water-ontology#Class> ;
    rdfs:label "Three Way Valve"^^xsd:string ;
    rdfs:subClassOf ns2:Valve .

<urn:nawi-water-ontology#TotalOrganicCompoundConcentrationSensor> a sh:NodeShape,
        <urn:nawi-water-ontology#Class> ;
    rdfs:label "TOC Sensor"^^xsd:string ;
    rdfs:comment "A sensor used to measure the total organic compound concentration"^^xsd:string ;
    rdfs:subClassOf <urn:nawi-water-ontology#ConcentrationSensor> .

<urn:nawi-water-ontology#TricklingFilter> a sh:NodeShape,
        <urn:nawi-water-ontology#Class> ;
    rdfs:label "TricklingFilter"^^xsd:string ;
    rdfs:comment "A filter system that treats wastewater by trickling it over a bed of rocks or plastic"^^xsd:string ;
    rdfs:subClassOf <urn:nawi-water-ontology#Filter>,
        <urn:nawi-water-ontology#UnitProcess> ;
    sh:property [ sh:hasValue <urn:nawi-water-ontology#Process-Biofiltration> ;
            sh:maxCount 1 ;
            sh:message "Instances of TricklingFilter must have the Biofiltration process."^^xsd:string ;
            sh:minCount 1 ;
            sh:path <urn:nawi-water-ontology#hasProcess> ] .

<urn:nawi-water-ontology#TurbidityMeter> a sh:NodeShape,
        <urn:nawi-water-ontology#Class> ;
    rdfs:label "TurbidityMeter"^^xsd:string ;
    rdfs:comment "A sensor used to measure the turbidity (clarity) of a fluid"^^xsd:string ;
    rdfs:subClassOf <urn:nawi-water-ontology#Sensor> .

<urn:nawi-water-ontology#UVH2O2Reactor> a sh:NodeShape,
        <urn:nawi-water-ontology#Class> ;
    rdfs:label "UV/H2O2 Reactor"^^xsd:string ;
    rdfs:comment "A specific reactor used in Advanced Oxidation Processes (AOPs) combining UV light with hydrogen peroxide."^^xsd:string ;
    rdfs:subClassOf <urn:nawi-water-ontology#Reactor>,
        <urn:nawi-water-ontology#UnitProcess> ;
    sh:property [ sh:hasValue <urn:nawi-water-ontology#Process-AdvancedOxidation> ;
            sh:maxCount 1 ;
            sh:message "Instances of UVH2O2Reactor must have the AdvancedOxidation process."^^xsd:string ;
            sh:minCount 1 ;
            sh:path <urn:nawi-water-ontology#hasProcess> ] .

<urn:nawi-water-ontology#UltrafiltrationUnit> a sh:NodeShape,
        <urn:nawi-water-ontology#Class> ;
    rdfs:label "UltrafiltrationUnit"^^xsd:string ;
    rdfs:comment "A filter system that uses a pressure-driven barrier to separate particles and solutes in a fluid"^^xsd:string ;
    rdfs:subClassOf <urn:nawi-water-ontology#Filter> .

<urn:nawi-water-ontology#UltravioletLightUnit> a sh:NodeShape,
        <urn:nawi-water-ontology#Class> ;
    rdfs:label "UltravioletlightUnit"^^xsd:string ;
    rdfs:comment "A unit using ultraviolet light for disinfection"^^xsd:string ;
    rdfs:subClassOf <urn:nawi-water-ontology#DisinfectionUnit> ;
    sh:property [ sh:hasValue <urn:nawi-water-ontology#Process-UVDisinfection> ;
            sh:maxCount 1 ;
            sh:message "Instances of UltravioletLightUnit must have the UVDisinfection process."^^xsd:string ;
            sh:minCount 1 ;
            sh:path <urn:nawi-water-ontology#hasProcess> ] .

<urn:nawi-water-ontology#Valve> a ns2:Class,
        sh:NodeShape,
        <urn:nawi-water-ontology#Class> ;
    rdfs:label "Valve"^^xsd:string ;
    rdfs:subClassOf ns2:Valve .

<urn:nawi-water-ontology#VariableFrequencyDrive> a ns2:Class,
        sh:NodeShape,
        <urn:nawi-water-ontology#Class> ;
    rdfs:label "Variable Frequency Drive"^^xsd:string ;
    rdfs:subClassOf ns2:VariableFrequencyDrive .

<urn:nawi-water-ontology#VolumeSensor> a sh:NodeShape,
        <urn:nawi-water-ontology#Class> ;
    rdfs:label "VolumeSensor"^^xsd:string ;
    rdfs:comment "A sensor used to measure the volume of a substance"^^xsd:string ;
    rdfs:subClassOf ns2:Sensor .

<urn:nawi-water-ontology#pHSensor> a sh:NodeShape,
        <urn:nawi-water-ontology#Class> ;
    rdfs:label "pHSensor"^^xsd:string ;
    rdfs:comment "A sensor used to measure the pH of a solution"^^xsd:string ;
    rdfs:subClassOf <urn:nawi-water-ontology#ConcentrationSensor> .

<urn:nawi-water-ontology/equip> rdfs:label "NAWI Water Equipment Ontology"^^xsd:string ;
    rdfs:comment "An ontology for water equipment used in the NAWI project"^^xsd:string ;
    owl:imports <http://data.ashrae.org/standard223/1.0/model/all> .

<urn:nawi-water-ontology/processtypes> rdfs:label "NAWI Water Process Types Ontology"^^xsd:string ;
    rdfs:comment "An ontology for types of unit process"^^xsd:string .

<urn:nawi-water-ontology/substances> rdfs:label "NAWI Water Substances Ontology"^^xsd:string ;
    rdfs:comment "An ontology for water substances used in the NAWI project"^^xsd:string ;
    owl:imports <http://data.ashrae.org/standard223/1.0/model/all> .

<urn:nawi-water-ontology#BeltThickener> a sh:NodeShape,
        <urn:nawi-water-ontology#Class> ;
    rdfs:label "BeltThickener"^^xsd:string ;
    rdfs:comment "A thickener that uses a belt system to separate solids from liquids"^^xsd:string ;
    rdfs:subClassOf <urn:nawi-water-ontology#Thickener>,
        <urn:nawi-water-ontology#UnitProcess> ;
    sh:property [ sh:hasValue <urn:nawi-water-ontology#Process-Filtration> ;
            sh:maxCount 1 ;
            sh:message "Instances of BeltThickener must have the Filtration process."^^xsd:string ;
            sh:minCount 1 ;
            sh:path <urn:nawi-water-ontology#hasProcess> ] .

<urn:nawi-water-ontology#Brine-15Percent> a sh:NodeShape,
        <urn:nawi-water-ontology#Brine-15Percent>,
        <urn:nawi-water-ontology#Class> ;
    rdfs:label "Brine-15Percent"^^xsd:string ;
    ns2:composedOf [ a ns2:QuantifiableProperty ;
            rdfs:label "Salt Concentration"^^xsd:string ;
            ns2:hasValue 15.0 ;
            ns2:ofConstituent <urn:nawi-water-ontology#Salt-NaCl> ;
            ns1:hasQuantityKind <http://qudt.org/vocab/quantitykind/MassFraction> ;
            ns1:hasUnit <http://qudt.org/vocab/unit/PERCENT> ],
        [ a ns2:QuantifiableProperty ;
            rdfs:label "Water Concentration"^^xsd:string ;
            ns2:hasValue 85.0 ;
            ns2:ofConstituent ns2:Constituent-H2O ;
            ns1:hasQuantityKind <http://qudt.org/vocab/quantitykind/MassFraction> ;
            ns1:hasUnit <http://qudt.org/vocab/unit/PERCENT> ] ;
    rdfs:comment "Brine-15Percent"^^xsd:string ;
    rdfs:subClassOf <urn:nawi-water-ontology#Water-Brine> .

<urn:nawi-water-ontology#Brine-5to10Percent> a sh:NodeShape,
        <urn:nawi-water-ontology#Brine-5to10Percent>,
        <urn:nawi-water-ontology#Class> ;
    rdfs:label "Brine-5to10Percent"^^xsd:string ;
    ns2:composedOf [ a ns2:QuantifiableProperty ;
            rdfs:label "High Salt Concentration"^^xsd:string ;
            ns2:hasAspect ns2:Aspect-HighLimit ;
            ns2:hasValue 10.0 ;
            ns2:ofConstituent <urn:nawi-water-ontology#Salt-NaCl> ;
            ns1:hasQuantityKind <http://qudt.org/vocab/quantitykind/MassFraction> ;
            ns1:hasUnit <http://qudt.org/vocab/unit/PERCENT> ],
        [ a ns2:QuantifiableProperty ;
            rdfs:label "Low Salt Concentration"^^xsd:string ;
            ns2:hasAspect ns2:Aspect-LowLimit ;
            ns2:hasValue 5.0 ;
            ns2:ofConstituent <urn:nawi-water-ontology#Salt-NaCl> ;
            ns1:hasQuantityKind <http://qudt.org/vocab/quantitykind/MassFraction> ;
            ns1:hasUnit <http://qudt.org/vocab/unit/PERCENT> ] ;
    rdfs:comment "Brine-5to10Percent"^^xsd:string ;
    rdfs:subClassOf <urn:nawi-water-ontology#Water-Brine> .

<urn:nawi-water-ontology#ChlorinationUnit> a sh:NodeShape,
        <urn:nawi-water-ontology#Class> ;
    rdfs:label "ChlorinationUnit"^^xsd:string ;
    rdfs:comment "A unit that uses chlorine or chlorine compounds for disinfection."^^xsd:string ;
    rdfs:subClassOf <urn:nawi-water-ontology#DisinfectionUnit> ;
    sh:property [ sh:hasValue <urn:nawi-water-ontology#Process-Chlorination> ;
            sh:maxCount 1 ;
            sh:message "Instances of ChlorinationUnit must have the Chlorination process."^^xsd:string ;
            sh:minCount 1 ;
            sh:path <urn:nawi-water-ontology#hasProcess> ] .

<urn:nawi-water-ontology#Coagulant-Alum> a sh:NodeShape,
        <urn:nawi-water-ontology#Class>,
        <urn:nawi-water-ontology#Coagulant-Alum> ;
    rdfs:label "Alum"^^xsd:string ;
    rdfs:comment "Aluminum sulfate (alum), a common coagulant"^^xsd:string ;
    rdfs:subClassOf <urn:nawi-water-ontology#Coagulant> .

<urn:nawi-water-ontology#Coagulant-FerricChloride> a sh:NodeShape,
        <urn:nawi-water-ontology#Class>,
        <urn:nawi-water-ontology#Coagulant-FerricChloride> ;
    rdfs:label "Ferric Chloride"^^xsd:string ;
    rdfs:comment "Ferric chloride, a coagulant for wastewater treatment"^^xsd:string ;
    rdfs:subClassOf <urn:nawi-water-ontology#Coagulant> .

<urn:nawi-water-ontology#Coagulant-PolyaluminumChloride> a sh:NodeShape,
        <urn:nawi-water-ontology#Class>,
        <urn:nawi-water-ontology#Coagulant-PolyaluminumChloride> ;
    rdfs:label "Polyaluminum Chloride"^^xsd:string ;
    rdfs:comment "Polyaluminum chloride (PAC), a coagulant"^^xsd:string ;
    rdfs:subClassOf <urn:nawi-water-ontology#Coagulant> .

<urn:nawi-water-ontology#Constituent-Metals> a sh:NodeShape,
        <urn:nawi-water-ontology#Class>,
        <urn:nawi-water-ontology#Constituent-Metals> ;
    rdfs:label "Constituent-Metals"^^xsd:string ;
    rdfs:comment "Constituent-Metals"^^xsd:string ;
    rdfs:subClassOf ns2:Medium-Constituent .

<urn:nawi-water-ontology#Constituent-Organics> a sh:NodeShape,
        <urn:nawi-water-ontology#Class>,
        <urn:nawi-water-ontology#Constituent-Organics> ;
    rdfs:label "Constituent-Organics"^^xsd:string ;
    rdfs:comment "Constituent-Organics"^^xsd:string ;
    rdfs:subClassOf ns2:Medium-Constituent .

<urn:nawi-water-ontology#Disinfectant-Chlorine> a sh:NodeShape,
        <urn:nawi-water-ontology#Class>,
        <urn:nawi-water-ontology#Disinfectant-Chlorine> ;
    rdfs:label "Chlorine"^^xsd:string ;
    rdfs:comment "Chlorine, a common disinfectant"^^xsd:string ;
    rdfs:subClassOf <urn:nawi-water-ontology#Disinfectant> .

<urn:nawi-water-ontology#Disinfectant-Ozone> a sh:NodeShape,
        <urn:nawi-water-ontology#Class>,
        <urn:nawi-water-ontology#Disinfectant-Ozone> ;
    rdfs:label "Ozone"^^xsd:string ;
    rdfs:comment "Ozone, an advanced disinfectant"^^xsd:string ;
    rdfs:subClassOf <urn:nawi-water-ontology#Disinfectant> .

<urn:nawi-water-ontology#Flocculant-Polyacrylamide> a sh:NodeShape,
        <urn:nawi-water-ontology#Class>,
        <urn:nawi-water-ontology#Flocculant-Polyacrylamide> ;
    rdfs:label "Polyacrylamide"^^xsd:string ;
    rdfs:comment "Polyacrylamide, a common flocculant"^^xsd:string ;
    rdfs:subClassOf <urn:nawi-water-ontology#Flocculant> .

<urn:nawi-water-ontology#Fluid-Sludge> a sh:NodeShape,
        <urn:nawi-water-ontology#Class>,
        <urn:nawi-water-ontology#Fluid-Sludge> ;
    rdfs:label "Sludge"^^xsd:string ;
    ns2:composedOf [ a ns2:QuantifiableProperty ;
            ns2:ofConstituent <urn:nawi-water-ontology#Constituent-Solids> ;
            ns1:hasQuantityKind <http://qudt.org/vocab/quantitykind/MassFraction> ;
            ns1:hasUnit <http://qudt.org/vocab/unit/PERCENT> ],
        [ a ns2:QuantifiableProperty ;
            ns2:ofConstituent ns2:Constituent-H2O ;
            ns1:hasQuantityKind <http://qudt.org/vocab/quantitykind/MassFraction> ;
            ns1:hasUnit <http://qudt.org/vocab/unit/PERCENT> ] ;
    rdfs:comment "A semi-solid slurry composed of water and solids."^^xsd:string ;
    rdfs:subClassOf ns2:Mix-Fluid .

<urn:nawi-water-ontology#HeavyMetalRemovalAgent-SodiumSulfide> a sh:NodeShape,
        <urn:nawi-water-ontology#Class>,
        <urn:nawi-water-ontology#HeavyMetalRemovalAgent-SodiumSulfide> ;
    rdfs:label "Sodium Sulfide"^^xsd:string ;
    rdfs:comment "Sodium sulfide, used to precipitate heavy metals"^^xsd:string ;
    rdfs:subClassOf <urn:nawi-water-ontology#HeavyMetalRemovalAgent> .

<urn:nawi-water-ontology#MediaFiltration> a sh:NodeShape,
        <urn:nawi-water-ontology#Class> ;
    rdfs:label "MediaFiltrationUnit"^^xsd:string ;
    rdfs:comment "A filter system that uses a bed of material to filter out contaminants"^^xsd:string ;
    rdfs:subClassOf <urn:nawi-water-ontology#Filter> .

<urn:nawi-water-ontology#OdorControlAgent-ActivatedCarbon> a sh:NodeShape,
        <urn:nawi-water-ontology#Class>,
        <urn:nawi-water-ontology#OdorControlAgent-ActivatedCarbon> ;
    rdfs:label "Activated Carbon"^^xsd:string ;
    rdfs:comment "Activated carbon, used to absorb odors"^^xsd:string ;
    rdfs:subClassOf <urn:nawi-water-ontology#OdorControlAgent> .

<urn:nawi-water-ontology#Process-ChemicalPrecipitation> a <urn:nawi-water-ontology#Class>,
        <urn:nawi-water-ontology#Process-ChemicalPrecipitation> ;
    rdfs:label "Chemical Precipitation"^^xsd:string ;
    rdfs:subClassOf <urn:nawi-water-ontology#Chemical-Process> ;
    skos:definition "Removal of nutrients or metals using coagulants"^^xsd:string .

<urn:nawi-water-ontology#Process-ClosedCircuitReverseOsmosis> a <urn:nawi-water-ontology#Class>,
        <urn:nawi-water-ontology#Process-ClosedCircuitReverseOsmosis> ;
    rdfs:label "Closed Circuit Reverse Osmosis (CCRO)"^^xsd:string ;
    rdfs:subClassOf <urn:nawi-water-ontology#Process-ReverseOsmosis> ;
    skos:definition "A specific RO configuration explored for optimization, capable of adapting to unmeasured changes like feed salinity."^^xsd:string .

<urn:nawi-water-ontology#Process-ElectroDialyticCrystallization> a <urn:nawi-water-ontology#Class>,
        <urn:nawi-water-ontology#Process-ElectroDialyticCrystallization> ;
    rdfs:label "Electro-Dialytic Crystallization (EDC)"^^xsd:string ;
    rdfs:subClassOf <urn:nawi-water-ontology#Process-Crystallization>,
        <urn:nawi-water-ontology#Process-Electrodialysis> ;
    skos:definition "A novel integrated process combining electrodialysis and crystallization for energy-efficient Zero-Liquid Discharge (ZLD) by maintaining a saturated brine stream."^^xsd:string .

<urn:nawi-water-ontology#Process-Electrooxidation> a <urn:nawi-water-ontology#Class>,
        <urn:nawi-water-ontology#Process-Electrooxidation> ;
    rdfs:label "Electrooxidation (EO)"^^xsd:string ;
    rdfs:subClassOf <urn:nawi-water-ontology#Physical-Process>,
        <urn:nawi-water-ontology#Process-Oxidation> ;
    skos:definition "An advanced oxidation process often combined with EC to enhance contaminant removal and inactivation, particularly for viruses."^^xsd:string .

<urn:nawi-water-ontology#Process-Equalization> a <urn:nawi-water-ontology#Class>,
        <urn:nawi-water-ontology#Process-Equalization> ;
    rdfs:label "Equalization"^^xsd:string ;
    rdfs:subClassOf <urn:nawi-water-ontology#Physical-Process> ;
    skos:definition "Flow and load dampening using a tank or basin"^^xsd:string .

<urn:nawi-water-ontology#Process-FeedReversalReverseOsmosis> a <urn:nawi-water-ontology#Class>,
        <urn:nawi-water-ontology#Process-FeedReversalReverseOsmosis> ;
    rdfs:label "Feed Reversal Reverse Osmosis (FRRO)"^^xsd:string ;
    rdfs:subClassOf <urn:nawi-water-ontology#Process-ReverseOsmosis> ;
    skos:definition "A dynamic and cyclic design to mitigate scaling and balance salt/foulant load, enabling high recovery."^^xsd:string .

<urn:nawi-water-ontology#Process-HighDensitySludge> a <urn:nawi-water-ontology#Class>,
        <urn:nawi-water-ontology#Process-HighDensitySludge> ;
    rdfs:label "High-Density Sludge (HDS) Process"^^xsd:string ;
    rdfs:subClassOf <urn:nawi-water-ontology#Chemical-Process>,
        <urn:nawi-water-ontology#Physical-Process> ;
    skos:definition "A method for treating acid mine drainage involving neutralization."^^xsd:string .

<urn:nawi-water-ontology#Process-MembraneDistillation> a <urn:nawi-water-ontology#Class>,
        <urn:nawi-water-ontology#Process-MembraneDistillation> ;
    rdfs:label "Membrane Distillation (MD)"^^xsd:string ;
    rdfs:subClassOf <urn:nawi-water-ontology#Process-MembraneProcess> ;
    skos:definition "A thermal membrane process, often subject to CFD modeling for optimization of heat and mass transfer."^^xsd:string .

<urn:nawi-water-ontology#Process-Neutralization> a <urn:nawi-water-ontology#Class>,
        <urn:nawi-water-ontology#Process-Neutralization> ;
    rdfs:label "Neutralization"^^xsd:string ;
    rdfs:subClassOf <urn:nawi-water-ontology#Process-pHAdjustment> ;
    skos:definition "pH adjustment, typically with a base, used in processes like high-density sludge treatment."^^xsd:string .

<urn:nawi-water-ontology#Process-OsmoticallyAssistedReverseOsmosis> a <urn:nawi-water-ontology#Class>,
        <urn:nawi-water-ontology#Process-OsmoticallyAssistedReverseOsmosis> ;
    rdfs:label "Osmotically Assisted Reverse Osmosis (OARO)"^^xsd:string ;
    rdfs:subClassOf <urn:nawi-water-ontology#Process-ReverseOsmosis> ;
    skos:definition "A process with validated Computational Fluid Dynamics (CFD) models for cost optimization."^^xsd:string .

<urn:nawi-water-ontology#Process-Reduction> a <urn:nawi-water-ontology#Class>,
        <urn:nawi-water-ontology#Process-Reduction> ;
    rdfs:label "Chemical Reduction"^^xsd:string ;
    rdfs:subClassOf <urn:nawi-water-ontology#Chemical-Process> ;
    skos:definition "Mechanism by which contaminants are transformed through the gain of electrons."^^xsd:string .

<urn:nawi-water-ontology#Process-Softening> a <urn:nawi-water-ontology#Class>,
        <urn:nawi-water-ontology#Process-Softening> ;
    rdfs:label "Softening"^^xsd:string ;
    rdfs:subClassOf <urn:nawi-water-ontology#Chemical-Process> ;
    skos:definition "Chemical precipitation of calcium/magnesium"^^xsd:string .

<urn:nawi-water-ontology#Sludge-MixedLiquor> a sh:NodeShape,
        <urn:nawi-water-ontology#Class>,
        <urn:nawi-water-ontology#Sludge-MixedLiquor> ;
    rdfs:label "Sludge-MixedLiquor"^^xsd:string ;
    ns2:composedOf [ a ns2:QuantifiableProperty ;
            rdfs:label "Suspended Solids Fraction"^^xsd:string ;
            ns2:ofConstituent <urn:nawi-water-ontology#Constituent-SuspendedSolids> ;
            ns1:hasQuantityKind <http://qudt.org/vocab/quantitykind/MassFraction> ;
            ns1:hasUnit <http://qudt.org/vocab/unit/PERCENT> ],
        [ a ns2:QuantifiableProperty ;
            rdfs:label "Water Fraction"^^xsd:string ;
            ns2:ofConstituent ns2:Constituent-H2O ;
            ns1:hasQuantityKind <http://qudt.org/vocab/quantitykind/MassFraction> ;
            ns1:hasUnit <http://qudt.org/vocab/unit/PERCENT> ] ;
    rdfs:comment "Mixed liquor is the mixture of wastewater and activated sludge in the aeration basin of a wastewater treatment plant. It contains suspended solids and water."^^xsd:string ;
    rdfs:subClassOf ns2:Fluid-Sludge .

<urn:nawi-water-ontology#hasAccuracy> a rdf:Property ;
    rdfs:label "has accuracy"^^xsd:string ;
    rdfs:comment "The `hasAccuracy` relation is used to link to a numerical `Property` whose value indicates the maximum expected deviation between the measured value and the true value in engineering units."^^xsd:string .

<urn:nawi-water-ontology#hasBias> a rdf:Property ;
    rdfs:label "has bias"^^xsd:string ;
    rdfs:comment "The `hasBias` relation is used to link to a numerical `Property` whose value indicates the systematic offset or drift in measurements relative to the true value."^^xsd:string .

<urn:nawi-water-ontology#hasCalibrationCurve> a rdf:Property ;
    rdfs:label "has calibration curve"^^xsd:string ;
    rdfs:comment "The `hasCalibrationCurve` relation is used to link to a `Property` that describes the mathematical relationship or lookup table between raw sensor output and calibrated engineering units."^^xsd:string .

<urn:nawi-water-ontology#hasDropRate> a rdf:Property ;
    rdfs:label "has drop rate"^^xsd:string ;
    rdfs:comment "The `hasDropRate` relation is used to link to a `Property` describes the amount of data points lost within a range of time due to latencies or other factors."^^xsd:string .

<urn:nawi-water-ontology#hasNumericRange> a rdf:Property ;
    rdfs:label "has numeric range"^^xsd:string ;
    rdfs:comment "The `hasNumericRange` relation is used to link to a numerical `Property` whose value indicates the span between the minimum and maximum measurable values in engineering units."^^xsd:string .

<urn:nawi-water-ontology#hasNumericResolution> a rdf:Property ;
    rdfs:label "has numeric resolution"^^xsd:string ;
    rdfs:comment "The `hasNumericResolution` relation is used to link to a numerical `Property` whose value indicates the smallest distinguishable difference between two measured values in engineering units."^^xsd:string .

<urn:nawi-water-ontology#hasPrecision> a rdf:Property ;
    rdfs:label "has precision"^^xsd:string ;
    rdfs:comment "The `hasPrecision` relation is used to link to a numerical `Property` whose value indicates the repeatability or reproducibility of measurements under identical conditions."^^xsd:string .

<urn:nawi-water-ontology#hasProcessedData> a rdf:Property ;
    rdfs:label "has processed data"^^xsd:string ;
    rdfs:comment "The `hasProcessedData` relation is used to link to a `Property` that describes any data processing, filtering, or transformation applied to the raw measurement values."^^xsd:string .

<urn:nawi-water-ontology#hasResponseTime> a rdf:Property ;
    rdfs:label "has response time"^^xsd:string ;
    rdfs:comment "The `hasResponseTime` relation is used to link to a numerical `Property` whose value indicates the time required for the sensor or measurement system to respond to a step change in the measured variable."^^xsd:string .

<urn:nawi-water-ontology#hasTemporalRange> a rdf:Property ;
    rdfs:label "has temporal range"^^xsd:string ;
    rdfs:comment "The `hasTemporalRange` relation is used to link to a numerical `Property` whose value indicates the start and end times for which data has been recorded."^^xsd:string .

<urn:nawi-water-ontology#hasTemporalResolution> a rdf:Property ;
    rdfs:label "has temporal resolution"^^xsd:string ;
    rdfs:comment "The `hasTemporalResolution` relation is used to link to a numerical `Property` whose value indicates the minimum time interval between successive measurements or data points."^^xsd:string .

<urn:nawi-water-ontology#hasVariableRange> a rdf:Property ;
    rdfs:label "has variable range"^^xsd:string ;
    rdfs:comment "The `hasVariableRange` relation is used to link to a numerical `Property` whose value indicates the expected range of variation for the measured variable under normal operating conditions."^^xsd:string .

<urn:nawi-water-ontology#pHAdjuster-Lime> a sh:NodeShape,
        <urn:nawi-water-ontology#Class>,
        <urn:nawi-water-ontology#pHAdjuster-Lime> ;
    rdfs:label "Lime"^^xsd:string ;
    rdfs:comment "Calcium hydroxide (lime), used to increase pH"^^xsd:string ;
    rdfs:subClassOf <urn:nawi-water-ontology#pHAdjuster> .

<urn:nawi-water-ontology#pHAdjuster-SulfuricAcid> a sh:NodeShape,
        <urn:nawi-water-ontology#Class>,
        <urn:nawi-water-ontology#pHAdjuster-SulfuricAcid> ;
    rdfs:label "Sulfuric Acid"^^xsd:string ;
    rdfs:comment "Sulfuric acid, used to decrease pH"^^xsd:string ;
    rdfs:subClassOf <urn:nawi-water-ontology#pHAdjuster> .

<urn:nawi-water-ontology#ConcentrationSensor> a sh:NodeShape,
        <urn:nawi-water-ontology#Class> ;
    rdfs:label "ConcentrationSensor"^^xsd:string ;
    rdfs:comment "A sensor used to measure the concentration of specific substances (e.g., Total Dissolved Solids)"^^xsd:string ;
    rdfs:subClassOf ns2:ConcentrationSensor .

<urn:nawi-water-ontology#Constituent-Salt> a sh:NodeShape,
        <urn:nawi-water-ontology#Class>,
        <urn:nawi-water-ontology#Constituent-Salt> ;
    rdfs:label "Constituent-Salt"^^xsd:string ;
    rdfs:comment "Constituent-Salt"^^xsd:string ;
    rdfs:subClassOf ns2:Medium-Constituent .

<urn:nawi-water-ontology#Constituent-SuspendedSolids> a sh:NodeShape,
        <urn:nawi-water-ontology#Class>,
        <urn:nawi-water-ontology#Constituent-SuspendedSolids> ;
    rdfs:label "Constituent-SuspendedSolids"^^xsd:string ;
    rdfs:comment "Suspended solids are particulate matter that is not dissolved in water and can be removed by filtration including organic and inorganic particles."^^xsd:string ;
    rdfs:subClassOf <urn:nawi-water-ontology#Constituent-Solids> .

<urn:nawi-water-ontology#Digester> a sh:NodeShape,
        <urn:nawi-water-ontology#Class> ;
    rdfs:label "Digester"^^xsd:string ;
    rdfs:comment "A container to promote decomposition of organic waste"^^xsd:string ;
    rdfs:subClassOf <urn:nawi-water-ontology#Tank> .

<urn:nawi-water-ontology#DisinfectionUnit> a sh:NodeShape,
        <urn:nawi-water-ontology#Class> ;
    rdfs:label "Disinfection"^^xsd:string ;
    rdfs:comment "A unit used to eliminate or reduce harmful microorganisms"^^xsd:string ;
    rdfs:subClassOf <urn:nawi-water-ontology#Tank>,
        <urn:nawi-water-ontology#UnitProcess> ;
    sh:property [ sh:hasValue <urn:nawi-water-ontology#Process-Disinfection> ;
            sh:maxCount 1 ;
            sh:message "Instances of DisinfectionUnit must have the Disinfection process."^^xsd:string ;
            sh:minCount 1 ;
            sh:path <urn:nawi-water-ontology#hasProcess> ] .

<urn:nawi-water-ontology#Electrode> a sh:NodeShape,
        <urn:nawi-water-ontology#Class> ;
    rdfs:label "Electrode"^^xsd:string ;
    rdfs:comment "A component where electrochemical reactions occur in electrified processes."^^xsd:string ;
    rdfs:subClassOf ns2:Equipment .

<urn:nawi-water-ontology#Flocculant> a sh:NodeShape,
        <urn:nawi-water-ontology#Class>,
        <urn:nawi-water-ontology#Flocculant> ;
    rdfs:label "Flocculant"^^xsd:string ;
    rdfs:comment "Class for flocculants used in wastewater treatment"^^xsd:string ;
    rdfs:subClassOf <urn:nawi-water-ontology#WastewaterTreatmentChemical> .

<urn:nawi-water-ontology#HeavyMetalRemovalAgent> a sh:NodeShape,
        <urn:nawi-water-ontology#Class>,
        <urn:nawi-water-ontology#HeavyMetalRemovalAgent> ;
    rdfs:label "Heavy Metal Removal Agent"^^xsd:string ;
    rdfs:comment "Class for chemicals used to remove heavy metals"^^xsd:string ;
    rdfs:subClassOf <urn:nawi-water-ontology#WastewaterTreatmentChemical> .

<urn:nawi-water-ontology#OdorControlAgent> a sh:NodeShape,
        <urn:nawi-water-ontology#Class>,
        <urn:nawi-water-ontology#OdorControlAgent> ;
    rdfs:label "Odor Control Agent"^^xsd:string ;
    rdfs:comment "Class for chemicals used for odor control"^^xsd:string ;
    rdfs:subClassOf <urn:nawi-water-ontology#WastewaterTreatmentChemical> .

<urn:nawi-water-ontology#Process-ActivatedSludge> a <urn:nawi-water-ontology#Class>,
        <urn:nawi-water-ontology#Process-ActivatedSludge> ;
    rdfs:label "Activated Sludge"^^xsd:string ;
    rdfs:subClassOf <urn:nawi-water-ontology#Biological-Process> ;
    skos:definition "Aerobic suspended-growth biological treatment"^^xsd:string .

<urn:nawi-water-ontology#Process-Adsorption> a <urn:nawi-water-ontology#Class>,
        <urn:nawi-water-ontology#Process-Adsorption> ;
    rdfs:label "Adsorption"^^xsd:string ;
    rdfs:subClassOf <urn:nawi-water-ontology#Physical-Process> ;
    skos:definition "A process by which substances bind to a surface."^^xsd:string .

<urn:nawi-water-ontology#Process-AdvancedOxidation> a <urn:nawi-water-ontology#Class>,
        <urn:nawi-water-ontology#Process-AdvancedOxidation> ;
    rdfs:label "Advanced Oxidation Process (AOP)"^^xsd:string ;
    rdfs:subClassOf <urn:nawi-water-ontology#Process-Oxidation> ;
    skos:definition "Processes combining UV light with oxidants (e.g., UV-AOP) to destroy contaminants."^^xsd:string .

<urn:nawi-water-ontology#Process-AerobicDigestion> a <urn:nawi-water-ontology#Class>,
        <urn:nawi-water-ontology#Process-AerobicDigestion> ;
    rdfs:label "Aerobic Digestion"^^xsd:string ;
    rdfs:subClassOf <urn:nawi-water-ontology#Biological-Process> ;
    skos:definition "A biological process that breaks down organic matter in the presence of oxygen."^^xsd:string .

<urn:nawi-water-ontology#Process-AnaerobicDigestion> a <urn:nawi-water-ontology#Class>,
        <urn:nawi-water-ontology#Process-AnaerobicDigestion> ;
    rdfs:label "Anaerobic Digestion"^^xsd:string ;
    rdfs:subClassOf <urn:nawi-water-ontology#Biological-Process> ;
    skos:definition "A biological process that breaks down organic matter in the absence of oxygen."^^xsd:string .

<urn:nawi-water-ontology#Process-BiologicallyActiveFiltration> a <urn:nawi-water-ontology#Class>,
        <urn:nawi-water-ontology#Process-BiologicallyActiveFiltration> ;
    rdfs:label "Biologically Active Filtration (BAF)"^^xsd:string ;
    rdfs:subClassOf <urn:nawi-water-ontology#Process-Biofiltration> ;
    skos:definition "A filtration method that uses biological processes to remove contaminants."^^xsd:string .

<urn:nawi-water-ontology#Process-Centrifugation> a <urn:nawi-water-ontology#Class>,
        <urn:nawi-water-ontology#Process-Centrifugation> ;
    rdfs:label "Centrifugation"^^xsd:string ;
    rdfs:subClassOf <urn:nawi-water-ontology#Physical-Process> ;
    skos:definition "A process that uses centrifugal force to separate substances of different densities."^^xsd:string .

<urn:nawi-water-ontology#Process-Chlorination> a <urn:nawi-water-ontology#Class>,
        <urn:nawi-water-ontology#Process-Chlorination> ;
    rdfs:label "Chlorination"^^xsd:string ;
    rdfs:subClassOf <urn:nawi-water-ontology#Process-Disinfection> ;
    skos:definition "A disinfection process that uses chlorine or chlorine compounds."^^xsd:string .

<urn:nawi-water-ontology#Process-Condensation> a <urn:nawi-water-ontology#Class>,
        <urn:nawi-water-ontology#Process-Condensation> ;
    rdfs:label "Condensation"^^xsd:string ;
    rdfs:subClassOf <urn:nawi-water-ontology#Physical-Process> ;
    skos:definition "A process of turning a vapor into a liquid."^^xsd:string .

<urn:nawi-water-ontology#Process-Dewatering> a <urn:nawi-water-ontology#Class>,
        <urn:nawi-water-ontology#Process-Dewatering> ;
    rdfs:label "Dewatering"^^xsd:string ;
    rdfs:subClassOf <urn:nawi-water-ontology#Physical-Process> ;
    skos:definition "A process to remove or separate water from another material, typically solids."^^xsd:string .

<urn:nawi-water-ontology#Process-Electrocoagulation> a <urn:nawi-water-ontology#Class>,
        <urn:nawi-water-ontology#Process-Electrocoagulation> ;
    rdfs:label "Electrocoagulation (EC)"^^xsd:string ;
    rdfs:subClassOf <urn:nawi-water-ontology#Physical-Process>,
        <urn:nawi-water-ontology#Process-Coagulation> ;
    skos:definition "An electrified pretreatment technology using sacrificial anodes to release coagulant precursors for contaminant removal."^^xsd:string .

<urn:nawi-water-ontology#Process-Electrolysis> a <urn:nawi-water-ontology#Class>,
        <urn:nawi-water-ontology#Process-Electrolysis> ;
    rdfs:label "Electrolysis"^^xsd:string ;
    rdfs:subClassOf <urn:nawi-water-ontology#Chemical-Process> ;
    skos:definition "A process that uses a direct electric current to drive an otherwise non-spontaneous chemical reaction."^^xsd:string .

<urn:nawi-water-ontology#Process-Evaporation> a <urn:nawi-water-ontology#Class>,
        <urn:nawi-water-ontology#Process-Evaporation> ;
    rdfs:label "Evaporation"^^xsd:string ;
    rdfs:subClassOf <urn:nawi-water-ontology#Physical-Process> ;
    skos:definition "A process of turning a liquid into a vapor."^^xsd:string .

<urn:nawi-water-ontology#Process-Flocculation> a <urn:nawi-water-ontology#Class>,
        <urn:nawi-water-ontology#Process-Flocculation> ;
    rdfs:label "Flocculation"^^xsd:string ;
    rdfs:subClassOf <urn:nawi-water-ontology#Chemical-Process> ;
    skos:definition "A unit process that gently mixes water to allow coagulated particles to form larger clumps."^^xsd:string .

<urn:nawi-water-ontology#Process-Flotation> a <urn:nawi-water-ontology#Class>,
        <urn:nawi-water-ontology#Process-Flotation> ;
    rdfs:label "Flotation"^^xsd:string ;
    rdfs:subClassOf <urn:nawi-water-ontology#Physical-Process> ;
    skos:definition "A unit process that uses buoyancy to separate solids from water, often using air bubbles."^^xsd:string .

<urn:nawi-water-ontology#Process-GasTransfer> a <urn:nawi-water-ontology#Class>,
        <urn:nawi-water-ontology#Process-GasTransfer> ;
    rdfs:label "Gas Transfer"^^xsd:string ;
    rdfs:subClassOf <urn:nawi-water-ontology#Physical-Process> ;
    skos:definition "A unit process that transfers gases, such as oxygen or carbon dioxide, into or out of water."^^xsd:string .

<urn:nawi-water-ontology#Process-GranulatedActivatedCarbonAdsorption> a <urn:nawi-water-ontology#Class>,
        <urn:nawi-water-ontology#Process-GranulatedActivatedCarbonAdsorption> ;
    rdfs:label "Granulated Activated Carbon Adsorption (GAC)"^^xsd:string ;
    rdfs:subClassOf <urn:nawi-water-ontology#Process-Adsorption> ;
    skos:definition "A process that uses activated carbon to adsorb impurities from water."^^xsd:string .

<urn:nawi-water-ontology#Process-IonExchange> a <urn:nawi-water-ontology#Class>,
        <urn:nawi-water-ontology#Process-IonExchange> ;
    rdfs:label "Ion Exchange"^^xsd:string ;
    rdfs:subClassOf <urn:nawi-water-ontology#Chemical-Process>,
        <urn:nawi-water-ontology#Physical-Process> ;
    skos:definition "A process in which ions are exchanged between a solution and an ion-exchange resin or membrane."^^xsd:string .

<urn:nawi-water-ontology#Process-MembraneBioreactor> a <urn:nawi-water-ontology#Class>,
        <urn:nawi-water-ontology#Process-MembraneBioreactor> ;
    rdfs:label "Membrane Bioreactor"^^xsd:string ;
    rdfs:subClassOf <urn:nawi-water-ontology#Biological-Process>,
        <urn:nawi-water-ontology#Physical-Process> ;
    skos:definition "Combined biological and membrane filtration"^^xsd:string .

<urn:nawi-water-ontology#Process-Mixing> a <urn:nawi-water-ontology#Class>,
        <urn:nawi-water-ontology#Process-Mixing> ;
    rdfs:label "Mixing"^^xsd:string ;
    rdfs:subClassOf <urn:nawi-water-ontology#Physical-Process> ;
    skos:definition "A unit process that mixes water with chemicals or other substances to achieve a desired effect."^^xsd:string .

<urn:nawi-water-ontology#Process-Ozonation> a <urn:nawi-water-ontology#Class>,
        <urn:nawi-water-ontology#Process-Ozonation> ;
    rdfs:label "Ozonation"^^xsd:string ;
    rdfs:subClassOf <urn:nawi-water-ontology#Process-Oxidation> ;
    skos:definition "A water treatment process that uses ozone as an oxidant."^^xsd:string .

<urn:nawi-water-ontology#Process-RapidSandFiltration> a <urn:nawi-water-ontology#Class>,
        <urn:nawi-water-ontology#Process-RapidSandFiltration> ;
    rdfs:label "Rapid Sand Filtration"^^xsd:string ;
    rdfs:subClassOf <urn:nawi-water-ontology#Process-Filtration> ;
    skos:definition "A filtration process that uses a bed of sand to remove impurities."^^xsd:string .

<urn:nawi-water-ontology#Process-Screening> a <urn:nawi-water-ontology#Class>,
        <urn:nawi-water-ontology#Process-Screening> ;
    rdfs:label "Screening"^^xsd:string ;
    rdfs:subClassOf <urn:nawi-water-ontology#Physical-Process> ;
    skos:definition "A unit process that removes large solids from water, such as leaves, branches, and other debris."^^xsd:string .

<urn:nawi-water-ontology#Process-SolventExtraction> a <urn:nawi-water-ontology#Class>,
        <urn:nawi-water-ontology#Process-SolventExtraction> ;
    rdfs:label "Solvent-Based Extraction"^^xsd:string ;
    rdfs:subClassOf <urn:nawi-water-ontology#Chemical-Process> ;
    skos:definition "A non-membrane, non-thermal method using a solvent to selectively extract water from highly saline brines."^^xsd:string .

<urn:nawi-water-ontology#Process-UVDisinfection> a <urn:nawi-water-ontology#Class>,
        <urn:nawi-water-ontology#Process-UVDisinfection> ;
    rdfs:label "UV Disinfection"^^xsd:string ;
    rdfs:subClassOf <urn:nawi-water-ontology#Physical-Process>,
        <urn:nawi-water-ontology#Process-Disinfection> ;
    skos:definition "A disinfection process that uses ultraviolet light to inactivate microorganisms."^^xsd:string .

<urn:nawi-water-ontology#Process-pHAdjustment> a <urn:nawi-water-ontology#Class>,
        <urn:nawi-water-ontology#Process-pHAdjustment> ;
    rdfs:label "pH Adjustment"^^xsd:string ;
    rdfs:subClassOf <urn:nawi-water-ontology#Chemical-Process> ;
    skos:definition "A unit process that adjusts the pH of water to a desired level using chemicals."^^xsd:string .

<urn:nawi-water-ontology#hasMeasurementRange> a rdf:Property ;
    rdfs:label "has measurement range"^^xsd:string ;
    rdfs:comment "The `hasMeasurementRange` relation is used to link to a numerical `Property` whose value indicates the expected range of variation that can physically be measured, e.g. by a sensor."^^xsd:string .

<urn:nawi-water-ontology#Constituent-Solids> a sh:NodeShape,
        <urn:nawi-water-ontology#Class>,
        <urn:nawi-water-ontology#Constituent-Solids> ;
    rdfs:label "Constituent-Solids"^^xsd:string ;
    rdfs:comment "Constituent-Solids"^^xsd:string ;
    rdfs:subClassOf ns2:Medium-Constituent .

<urn:nawi-water-ontology#Disinfectant> a sh:NodeShape,
        <urn:nawi-water-ontology#Class>,
        <urn:nawi-water-ontology#Disinfectant> ;
    rdfs:label "Disinfectant"^^xsd:string ;
    rdfs:comment "Class for disinfectants used in wastewater treatment"^^xsd:string ;
    rdfs:subClassOf <urn:nawi-water-ontology#WastewaterTreatmentChemical> .

<urn:nawi-water-ontology#Process-Biofiltration> a <urn:nawi-water-ontology#Class>,
        <urn:nawi-water-ontology#Process-Biofiltration> ;
    rdfs:label "Biofiltration"^^xsd:string ;
    rdfs:subClassOf <urn:nawi-water-ontology#Biological-Process>,
        <urn:nawi-water-ontology#Physical-Process> ;
    skos:definition "Fixed-film biological treatment (e.g., trickling filter)"^^xsd:string .

<urn:nawi-water-ontology#Process-Coagulation> a <urn:nawi-water-ontology#Class>,
        <urn:nawi-water-ontology#Process-Coagulation> ;
    rdfs:label "Coagulation"^^xsd:string ;
    rdfs:subClassOf <urn:nawi-water-ontology#Chemical-Process> ;
    skos:definition "A unit process that adds chemicals to water to cause small particles to clump together."^^xsd:string .

<urn:nawi-water-ontology#Process-MembraneProcess> a <urn:nawi-water-ontology#Class>,
        <urn:nawi-water-ontology#Process-MembraneProcess> ;
    rdfs:label "Membrane Process"^^xsd:string ;
    rdfs:subClassOf <urn:nawi-water-ontology#Physical-Process> ;
    skos:definition "A process that uses a semi-permeable membrane to separate substances."^^xsd:string .

<urn:nawi-water-ontology#Water-Brine> a sh:NodeShape,
        <urn:nawi-water-ontology#Class>,
        <urn:nawi-water-ontology#Water-Brine> ;
    rdfs:label "Water-Brine"^^xsd:string ;
    ns2:composedOf [ a ns2:QuantifiableProperty ;
            ns2:ofConstituent ns2:Constituent-H2O ;
            ns1:hasQuantityKind <http://qudt.org/vocab/quantitykind/MassFraction> ;
            ns1:hasUnit <http://qudt.org/vocab/unit/PERCENT> ],
        [ a ns2:QuantifiableProperty ;
            ns2:ofConstituent <urn:nawi-water-ontology#Salt-NaCl> ;
            ns1:hasQuantityKind <http://qudt.org/vocab/quantitykind/MassFraction> ;
            ns1:hasUnit <http://qudt.org/vocab/unit/PERCENT> ] ;
    rdfs:comment "Water-Brine"^^xsd:string ;
    rdfs:subClassOf ns2:Fluid-Water .

<urn:nawi-water-ontology#pHAdjuster> a sh:NodeShape,
        <urn:nawi-water-ontology#Class>,
        <urn:nawi-water-ontology#pHAdjuster> ;
    rdfs:label "pH Adjuster"^^xsd:string ;
    rdfs:comment "Class for pH adjusters used in wastewater treatment"^^xsd:string ;
    rdfs:subClassOf <urn:nawi-water-ontology#WastewaterTreatmentChemical> .

<urn:nawi-water-ontology#Basin> a sh:NodeShape,
        <urn:nawi-water-ontology#Class> ;
    rdfs:label "Basin"^^xsd:string ;
    rdfs:comment "A Basin is a physical structure or containment unit designed to hold and condition a volume of water as part of a treatment process. It has at least one inlet and one outlet for water flow and may include drains, overflow paths, mixing devices, or aeration elements depending on its operational role."^^xsd:string ;
    rdfs:subClassOf ns2:Equipment ;
    sh:property [ rdfs:comment "A basin has an inlet fluid connection point"^^xsd:string ;
            sh:path ns2:hasConnectionPoint ;
            sh:qualifiedMinCount 1 ;
            sh:qualifiedValueShape [ sh:class ns2:InletConnectionPoint ;
                    sh:property [ sh:hasValue ns2:Mix-Fluid ;
                            sh:path ns2:hasMedium ] ] ],
        [ rdfs:comment "A basin may have an overflow connection point"^^xsd:string ;
            sh:path ns2:hasConnectionPoint ;
            sh:qualifiedMinCount 0 ;
            sh:qualifiedValueShape [ sh:class ns2:OutletConnectionPoint ;
                    sh:property [ sh:hasValue ns2:Mix-Fluid ;
                            sh:path ns2:hasMedium ],
                        [ sh:hasValue ns2:Role-Overflow ;
                            sh:path ns2:hasRole ] ] ],
        [ rdfs:comment "A basin may have an drain connection point"^^xsd:string ;
            sh:path ns2:hasConnectionPoint ;
            sh:qualifiedMinCount 0 ;
            sh:qualifiedValueShape [ sh:class ns2:OutletConnectionPoint ;
                    sh:property [ sh:hasValue ns2:Role-Drain ;
                            sh:path ns2:hasRole ],
                        [ sh:hasValue ns2:Mix-Fluid ;
                            sh:path ns2:hasMedium ] ] ],
        [ rdfs:comment "A basin has an outlet fluid connection point"^^xsd:string ;
            sh:path ns2:hasConnectionPoint ;
            sh:qualifiedMinCount 1 ;
            sh:qualifiedValueShape [ sh:class ns2:OutletConnectionPoint ;
                    sh:property [ sh:hasValue ns2:Mix-Fluid ;
                            sh:path ns2:hasMedium ] ] ] .

<urn:nawi-water-ontology#Coagulant> a sh:NodeShape,
        <urn:nawi-water-ontology#Class>,
        <urn:nawi-water-ontology#Coagulant> ;
    rdfs:label "Coagulant"^^xsd:string ;
    rdfs:comment "Class for coagulants used in wastewater treatment"^^xsd:string ;
    rdfs:subClassOf <urn:nawi-water-ontology#WastewaterTreatmentChemical> .

<urn:nawi-water-ontology#Process-Crystallization> a <urn:nawi-water-ontology#Class>,
        <urn:nawi-water-ontology#Process-Crystallization> ;
    rdfs:label "Crystallization"^^xsd:string ;
    rdfs:subClassOf <urn:nawi-water-ontology#Physical-Process> ;
    skos:definition "A process of forming solid crystals from a solution."^^xsd:string .

<urn:nawi-water-ontology#Process-Disinfection> a <urn:nawi-water-ontology#Class>,
        <urn:nawi-water-ontology#Process-Disinfection> ;
    rdfs:label "Disinfection"^^xsd:string ;
    rdfs:subClassOf <urn:nawi-water-ontology#Chemical-Process> ;
    skos:definition "A unit process that uses chemicals or other methods to kill or inactivate harmful microorganisms in water."^^xsd:string .

<urn:nawi-water-ontology#Process-Electrodialysis> a <urn:nawi-water-ontology#Class>,
        <urn:nawi-water-ontology#Process-Electrodialysis> ;
    rdfs:label "Electrodialysis"^^xsd:string ;
    rdfs:subClassOf <urn:nawi-water-ontology#Chemical-Process>,
        <urn:nawi-water-ontology#Physical-Process> ;
    skos:definition "A process that uses ion-exchange membranes and an electric potential to separate ions from water."^^xsd:string .

<urn:nawi-water-ontology#Process-Oxidation> a <urn:nawi-water-ontology#Class>,
        <urn:nawi-water-ontology#Process-Oxidation> ;
    rdfs:label "Oxidation"^^xsd:string ;
    rdfs:subClassOf <urn:nawi-water-ontology#Chemical-Process> ;
    skos:definition "A unit process that adds oxidizing agents to water to remove contaminants or improve water quality."^^xsd:string .

<urn:nawi-water-ontology#Process-ReverseOsmosis> a <urn:nawi-water-ontology#Class>,
        <urn:nawi-water-ontology#Process-ReverseOsmosis> ;
    rdfs:label "Reverse Osmosis (RO)"^^xsd:string ;
    rdfs:subClassOf <urn:nawi-water-ontology#Process-MembraneProcess> ;
    skos:definition "A core membrane separation process for desalination and advanced purification."^^xsd:string .

<urn:nawi-water-ontology#Process-Sedimentation> a <urn:nawi-water-ontology#Class>,
        <urn:nawi-water-ontology#Process-Sedimentation> ;
    rdfs:label "Sedimentation"^^xsd:string ;
    rdfs:subClassOf <urn:nawi-water-ontology#Physical-Process> ;
    skos:definition "A unit process that allows solids to settle out of water by gravity."^^xsd:string .

<urn:nawi-water-ontology#Tank> a sh:NodeShape,
        <urn:nawi-water-ontology#Class> ;
    rdfs:label "Tank"^^xsd:string ;
    rdfs:comment "A tank for storing liquid"^^xsd:string ;
    rdfs:subClassOf ns2:Equipment ;
    sh:property [ rdfs:comment "A tank has an inlet fluid connection point"^^xsd:string ;
            sh:path ns2:hasConnectionPoint ;
            sh:qualifiedMinCount 1 ;
            sh:qualifiedValueShape [ sh:class ns2:InletConnectionPoint ;
                    sh:property [ sh:hasValue ns2:Mix-Fluid ;
                            sh:path ns2:hasMedium ] ] ],
        [ rdfs:comment "A tank has an outlet fluid connection point"^^xsd:string ;
            sh:path ns2:hasConnectionPoint ;
            sh:qualifiedMinCount 1 ;
            sh:qualifiedValueShape [ sh:class ns2:OutletConnectionPoint ;
                    sh:property [ sh:hasValue ns2:Mix-Fluid ;
                            sh:path ns2:hasMedium ] ] ] .

<urn:nawi-water-ontology#Process-Filtration> a <urn:nawi-water-ontology#Class>,
        <urn:nawi-water-ontology#Process-Filtration> ;
    rdfs:label "Filtration"^^xsd:string ;
    rdfs:subClassOf <urn:nawi-water-ontology#Physical-Process> ;
    skos:definition "A unit process that removes smaller particles from water by passing it through a filter."^^xsd:string .

<urn:nawi-water-ontology#Salt-NaCl> a sh:NodeShape,
        <urn:nawi-water-ontology#Class>,
        <urn:nawi-water-ontology#Salt-NaCl> ;
    rdfs:label "Salt-NaCl"^^xsd:string ;
    rdfs:comment "Salt-NaCl"^^xsd:string ;
    rdfs:subClassOf <urn:nawi-water-ontology#Constituent-Salt> .

<urn:nawi-water-ontology#Thickener> a sh:NodeShape,
        <urn:nawi-water-ontology#Class> ;
    rdfs:label "Thickener"^^xsd:string ;
    rdfs:comment "A device used to increase the solids concentration of a slurry"^^xsd:string ;
    rdfs:subClassOf ns2:Equipment .

<urn:nawi-water-ontology#Biological-Process> a <urn:nawi-water-ontology#Biological-Process>,
        <urn:nawi-water-ontology#Class> ;
    rdfs:label "Biological Process"^^xsd:string ;
    rdfs:subClassOf <urn:nawi-water-ontology#Process> ;
    skos:definition "A unit process that utilizes biological activity for water treatment."^^xsd:string .

<urn:nawi-water-ontology#Reactor> a sh:NodeShape,
        <urn:nawi-water-ontology#Class> ;
    rdfs:label "Reactor"^^xsd:string ;
    rdfs:comment "An equipment used for chemical reaction"^^xsd:string ;
    rdfs:subClassOf <urn:nawi-water-ontology#Tank> ;
    sh:property [ rdfs:comment "A reactor has at least one inlet fluid connection point"^^xsd:string ;
            sh:path ns2:hasConnectionPoint ;
            sh:qualifiedMinCount 1 ;
            sh:qualifiedValueShape [ sh:class ns2:InletConnectionPoint ;
                    sh:property [ sh:hasValue ns2:Mix-Fluid ;
                            sh:path ns2:hasMedium ] ] ],
        [ rdfs:comment "A reactor has at least one outlet fluid connection point"^^xsd:string ;
            sh:path ns2:hasConnectionPoint ;
            sh:qualifiedMinCount 1 ;
            sh:qualifiedValueShape [ sh:class ns2:OutletConnectionPoint ;
                    sh:property [ sh:hasValue ns2:Mix-Fluid ;
                            sh:path ns2:hasMedium ] ] ] .

<urn:nawi-water-ontology#WastewaterTreatmentChemical> a sh:NodeShape,
        <urn:nawi-water-ontology#Class>,
        <urn:nawi-water-ontology#WastewaterTreatmentChemical> ;
    rdfs:label "Wastewater Treatment Chemical"^^xsd:string ;
    rdfs:comment "Base class for all chemicals used in wastewater treatment"^^xsd:string ;
    rdfs:subClassOf ns2:Medium-Constituent .

ns2:Sensor sh:property [ rdfs:comment "The `hasMeasurementRange` relation is used to link to a numerical `Property` whose value indicates the maximum or minimum that can physically be measured, e.g. by a sensor."^^xsd:string ;
            sh:class ns2:QuantifiableProperty ;
            sh:path <urn:nawi-water-ontology#hasMeasurementRange> ] .

<urn:nawi-water-ontology#Filter> a sh:NodeShape,
        <urn:nawi-water-ontology#Class> ;
    rdfs:label "Filter"^^xsd:string ;
    rdfs:comment "An equipment used to remove impurities from liquids or gases"^^xsd:string ;
    rdfs:subClassOf ns2:Filter,
        <urn:nawi-water-ontology#UnitProcess> ;
    sh:property [ sh:hasValue <urn:nawi-water-ontology#Process-Filtration> ;
            sh:maxCount 1 ;
            sh:message "Instances of Filter must have the Filtration process."^^xsd:string ;
            sh:minCount 1 ;
            sh:path <urn:nawi-water-ontology#hasProcess> ] .

<urn:nawi-water-ontology#Chemical-Process> a <urn:nawi-water-ontology#Chemical-Process>,
        <urn:nawi-water-ontology#Class> ;
    rdfs:label "Chemical Process"^^xsd:string ;
    rdfs:subClassOf <urn:nawi-water-ontology#Process> ;
    skos:definition "A unit process that involves the addition of chemicals to water to achieve a desired effect."^^xsd:string .

<urn:nawi-water-ontology#Physical-Process> a <urn:nawi-water-ontology#Class>,
        <urn:nawi-water-ontology#Physical-Process> ;
    rdfs:label "Physical Process"^^xsd:string ;
    rdfs:subClassOf <urn:nawi-water-ontology#Process> ;
    skos:definition "A unit process that relies on physical forces to separate or treat water."^^xsd:string .

ns2:QuantifiableProperty sh:property [ rdfs:comment "The `hasPrecision` relation is used to link to a numerical `Property` whose value indicates the repeatability or reproducibility of measurements under identical conditions."^^xsd:string ;
            sh:class ns2:QuantifiableProperty ;
            sh:path <urn:nawi-water-ontology#hasPrecision> ],
        [ rdfs:comment "The `hasResponseTime` relation is used to link to a numerical `Property` whose value indicates the time required for the sensor or measurement system to respond to a step change in the measured variable."^^xsd:string ;
            sh:class ns2:QuantifiableProperty ;
            sh:path <urn:nawi-water-ontology#hasResponseTime> ],
        [ rdfs:comment "The `hasTemporalResolution` relation is used to link to a numerical `Property` whose value indicates the minimum time interval between successive measurements or data points."^^xsd:string ;
            sh:class ns2:QuantifiableProperty ;
            sh:path <urn:nawi-water-ontology#hasTemporalResolution> ],
        [ rdfs:comment "The `hasCalibrationCurve` relation is used to link to a `Property` that describes the mathematical relationship or lookup table between raw sensor output and calibrated engineering units."^^xsd:string ;
            sh:class ns2:QuantifiableProperty ;
            sh:path <urn:nawi-water-ontology#hasCalibrationCurve> ],
        [ rdfs:comment "The `hasNumericResolution` relation is used to link to a numerical `Property` whose value indicates the smallest distinguishable difference between two measured values in engineering units."^^xsd:string ;
            sh:class ns2:QuantifiableProperty ;
            sh:path <urn:nawi-water-ontology#hasNumericResolution> ],
        [ rdfs:comment "The `hasDropRate` relation is used to link to a `Property` describes the amount of data points lost within a range of time due to latencies or other factors."^^xsd:string ;
            sh:class ns2:QuantifiableProperty ;
            sh:path <urn:nawi-water-ontology#hasDropRate> ],
        [ rdfs:comment "The `hasMeasurementRange` relation is used to link to a numerical `Property` whose value indicates the maximum or minimum that can physically be measured, e.g. by a sensor."^^xsd:string ;
            sh:class ns2:QuantifiableProperty ;
            sh:path <urn:nawi-water-ontology#hasMeasurementRange> ],
        [ rdfs:comment "The `hasBias` relation is used to link to a numerical `Property` whose value indicates the systematic offset or drift in measurements relative to the true value."^^xsd:string ;
            sh:class ns2:QuantifiableProperty ;
            sh:path <urn:nawi-water-ontology#hasBias> ],
        [ rdfs:comment "The `hasAccuracy` relation is used to link to a numerical `Property` whose value indicates the maximum expected deviation between the measured value and the true value in engineering units."^^xsd:string ;
            sh:class ns2:QuantifiableProperty ;
            sh:path <urn:nawi-water-ontology#hasAccuracy> ],
        [ rdfs:comment "The `hasNumericRange` relation is used to link to a numerical `Property` whose value indicates the span between the minimum and maximum measured values."^^xsd:string ;
            sh:class ns2:QuantifiableProperty ;
            sh:path <urn:nawi-water-ontology#hasNumericRange> ],
        [ rdfs:comment "The `hasVariableRange` relation is used to link to a numerical `Property` whose value indicates the maximum or minimum for the measured variable during normal operation."^^xsd:string ;
            sh:class ns2:QuantifiableProperty ;
            sh:path <urn:nawi-water-ontology#hasVariableRange> ],
        [ rdfs:comment "The `hasTemporalRange` relation is used to link to a numerical `Property` whose value indicates the start and end times for which data has been recorded."^^xsd:string ;
            sh:class ns2:QuantifiableProperty ;
            sh:path <urn:nawi-water-ontology#hasTemporalRange> ],
        [ rdfs:comment "The `hasProcessedData` relation is used to link to a `Property` that describes any data processing, filtering, or transformation applied to the raw measurement values."^^xsd:string ;
            sh:class ns2:QuantifiableProperty ;
            sh:path <urn:nawi-water-ontology#hasProcessedData> ] .

<urn:nawi-water-ontology#hasProcess> a rdf:Property ;
    rdfs:label "has process"^^xsd:string ;
    rdfs:comment "This property is used to associate a water treatment process with a piece of equipment."^^xsd:string .

